save

Protocols/ABC/Pro.v
@@ -1,8 +1,10 @@
-From Coq Require Import Bool List.
+From Coq Require Import Bool List PeanoNat.
 From Coq Require ssrbool.
 Import (coercions) ssrbool.
 From ABCProtocol.Systems Require Export Protocol.
 From ABCProtocol.Protocols.ABC Require Export Types.
+
+From RecordUpdate Require Import RecordUpdate.
 
 Module Type ACProtocol (A : NetAddr) (V : Signable) (VBFT : ValueBFT A V) 
   (BTh : ByzThreshold A)
@@ -53,6 +55,9 @@ Record State_ :=
     (* TODO add it here, or in a separate State type? *)
     msg_buffer : list (Address * Message)
   }.
+
+#[export] Instance eta : Settable _ := settable! Node <id; conf; submitted_value; from_set; collected_lightsigs; 
+  collected_sigs; received_lightcerts; received_certs; msg_buffer>.
 
 Definition State := State_.
 (*
@@ -116,102 +121,106 @@ Definition routine_check (st : State) : list Packet :=
   match ov with 
   | Some vthis => 
     (* actually confirmation implies submission; but we need to use vthis so anyway *)
-    if conf
-    then 
-      (if lightcert_conflict_check rlcerts
-      then broadcast n (ConfirmMsg (vthis, zip_from_sigs st))
-      else nil)
+    if conf && (lightcert_conflict_check rlcerts)
+    then broadcast n (ConfirmMsg (vthis, zip_from_sigs st))
     else nil
   | None => nil
   end
 .
 
-Definition procMsg (st : State) (src : Address) (msg : Message) : State * list Packet :=
-  let: Node n conf ov from lsigs sigs rlcerts rcerts buffer := st in
+Definition procMsg (st : State) (src : Address) (msg : Message) : option (State * list Packet) :=
+  let: Node n cf ov from lsigs sigs rlcerts rcerts buffer := st in
   match msg with
   | SubmitMsg v lsig sig =>
     match ov with 
     | Some vthis => 
-      if Value_eqdec v vthis 
+      if (Value_eqdec v vthis) && (verify v sig src) && (light_verify v lsig src)
       then
-        (* just to clarify: in the paper, this check is subsumed by Line 6 *)
-        (if verify v sig src
-        then 
-          (if light_verify v lsig src
-          then 
-            (* before prepending, add a check to avoid adding a duplicate node-signature pair *)
-            (* checking In fst or In pair should be the same, due to the correctness of verify *)
-            (* prevent enlarging from_set after confirmation; TODO need to align this with paper? seems not ... *)
-            (* let: in_from := In_dec Address_eqdec src (map fst nsigs) in *)
-            let: in_from := In_dec Address_eqdec src from in
-            let: from' := if conf || in_from then from else src :: from in
-            let: lsigs' := if conf || in_from then lsigs else lsig :: lsigs in
-            let: sigs' := if conf || in_from then sigs else sig :: sigs in
-            (* let: conf' := (Nat.leb (N - t0) (length from')) in *)
-            let: conf' := conf || (Nat.leb (N - t0) (length from')) in
-            let: ps := (if conf' 
-              then broadcast n (LightConfirmMsg (v, lightsig_combine lsigs'))
-              else nil) in
-            let: st' := Node n conf' ov from' lsigs' sigs' rlcerts rcerts buffer in
-            (st', ps)
-          else (st, nil))
-        else (st, nil))
-      else (st, nil)
+        (* before prepending, add a check to avoid adding a duplicate node-signature pair *)
+        (* checking In fst or In pair should be the same, due to the correctness of verify *)
+        (* prevent enlarging from_set after confirmation; TODO need to align this with paper? seems not ... *)
+        (*
+        let: cond := cf || (in_dec Address_eqdec src from) in
+        let: from' := if cond then from else src :: from in
+        let: lsigs' := if cond then lsigs else lsig :: lsigs in
+        let: sigs' := if cond then sigs else sig :: sigs in
+        let: cf' := cf || ((N - t0) <=? (length from')) in
+        let: ps := (if cf'
+          then broadcast n (LightConfirmMsg (v, lightsig_combine lsigs'))
+          else nil) in
+        let: st' := st <| conf := cf' |> <| from_set := from' |>
+          <| collected_lightsigs := lsigs' |> <| collected_sigs := sigs' |> in
+        Some (st', ps)
+        *)
+        (* FIXME: the broadcast here can be implemented as a check, though *)
+        if cf
+        then Some (st, broadcast n (LightConfirmMsg (v, lightsig_combine lsigs)))
+        else 
+          if in_dec Address_eqdec src from
+          then None
+          else
+            let: cf' := (N - t0 <=? S (length from)) in
+            let: ps' := if cf' then broadcast n (LightConfirmMsg (v, lightsig_combine (lsig :: lsigs))) else nil in
+            let: st' := st <| conf := cf' |> <| from_set := src :: from |>
+              <| collected_lightsigs := lsig :: lsigs |> <| collected_sigs := sig :: sigs |> in
+            Some (st', ps')
+      else None
     | None => 
       (* add to the buffer and wait *)
-      (Node n conf ov from lsigs sigs rlcerts rcerts ((src, msg) :: buffer), nil)
+      let: st' := st <| msg_buffer := (src, msg) :: buffer |> in
+      Some (st', nil)
     end
   | LightConfirmMsg lc =>
     let: (v, cs) := lc in
     if combined_verify v cs
     then 
-      let: st' := Node n conf ov from lsigs sigs (lc :: rlcerts) rcerts buffer in
-      (st', nil)
-    else (st, nil)
+      let: st' := st <| received_lightcerts := lc :: rlcerts |> in
+      Some (st', nil)
+    else None
   | ConfirmMsg c => 
     let: (v, nsigs) := c in
     (* check whether this is a valid full certificate or not *)
     (* in the paper this condition is ">= N-t0 distinct senders", 
         which is stronger than this *)
-    if NoDup_eqdec AddrSigPair_eqdec nsigs
-    then 
-      (if Nat.leb (N - t0) (length nsigs) 
-      then
-        (if verify_certificate v nsigs
-        then 
-          let: st' := Node n conf ov from lsigs sigs rlcerts (c :: rcerts) buffer in
-          (st', nil)
-        else (st, nil))
-      else (st, nil))
-    else (st, nil)
+    if (NoDup_eqdec AddrSigPair_eqdec nsigs) && ((N - t0) <=? (length nsigs)) && (verify_certificate v nsigs)
+    then
+      let: st' := st <| received_certs := c :: rcerts |> in
+      Some (st', nil)
+    else None
   end.
 
 (* a simple wrapper *)
 
 Definition procMsgWithCheck (st : State) (src : Address) (msg : Message) : State * list Packet :=
-  let: (st', ps) := procMsg st src msg in
-  (* a minor optimization? *)
-  match msg with
-  | SubmitMsg _ _ _ | LightConfirmMsg _ => (st', routine_check st' ++ ps)
-  | _ => (st', ps)
+  match procMsg st src msg with
+  | Some (st', ps) =>
+    match msg with
+    | SubmitMsg _ _ _ | LightConfirmMsg _ => (st', routine_check st' ++ ps)
+    | _ => (st', ps)
+    end
+  | None => (st, nil) (* if the internal state does not change, then no need to do routine check *)
   end.
 
 Definition procInt (st : State) (tr : InternalTransition) :=
-  let: Node n conf ov from lsigs sigs rlcerts rcerts buffer := st in
+  let: Node n cf ov from lsigs sigs rlcerts rcerts buffer := st in
   match tr with
   | SubmitIntTrans => 
-    (* TODO constrain this to happen at most once? *)
-    let: vthis := value_bft n in
-    let: ps := broadcast n 
-      (SubmitMsg vthis (light_sign vthis (lightkey_map n)) (sign vthis (key_map n))) in
-    (* also start to process all messages in the buffer *)
-    (* not putting ps into the initial value of fold should be easier? *)
-    let: (st', ps') := 
-      fold_right
-        (fun nmsg stps => let: (res1, res2) := procMsgWithCheck (fst stps) (fst nmsg) (snd nmsg) in
-          (res1, res2 ++ snd stps)) 
-        (Node n conf (Some vthis) from lsigs sigs rlcerts rcerts nil, nil) buffer in
-    (st', ps' ++ ps)  
+    (* making it happen at most once should make things easier *)
+    match ov with
+    | None =>
+      let: vthis := value_bft n in
+      let: ps := broadcast n 
+        (SubmitMsg vthis (light_sign vthis (lightkey_map n)) (sign vthis (key_map n))) in
+      let: st_start := st <| submitted_value := Some vthis |> <| msg_buffer := nil |> in
+      (* also start to process all messages in the buffer *)
+      (* not putting ps into the initial value of fold should be easier? *)
+      let: (st', ps') := 
+        fold_right
+          (fun nmsg stps => let: (res1, res2) := procMsgWithCheck (fst stps) (fst nmsg) (snd nmsg) in
+            (res1, res2 ++ snd stps)) (st_start, nil) buffer in
+      (st', ps' ++ ps)
+    | Some _ => (st, nil)
+    end
   end.
 
 End ACProtocol.
