Protocols/ABC/Inv.v
@@ -1,0 +1,1946 @@
+From Coq Require Import List Bool Lia PeanoNat ListSet Permutation RelationClasses.
+From Coq Require ssrbool ssreflect.
+Import (coercions) ssrbool.
+Import ssreflect.SsrSyntax.
+From ABCProtocol.Protocols.ABC Require Export Nw.
+
+From RecordUpdate Require Import RecordUpdate.
+From stdpp Require Import tactics. (* anyway *)
+
+Module ACInvariant (A : NetAddr) (V : Signable) (VBFT : ValueBFT A V) 
+  (BTh : ByzThreshold A) (BSett : ByzSetting A)
+  (P : PKI A V) (TSS : ThresholdSignatureScheme A V with Definition thres := BTh.t0).
+
+Import A V VBFT BTh BSett P TSS.
+Import ssrbool. (* anyway *)
+
+Module Export ACN := ACNetwork A V VBFT BTh BSett P TSS.
+
+Definition id_coh w : Prop := forall n, (w @ n).(id) = n.
+
+(* state invariants *)
+
+Notation NoDup := List.NoDup.
+
+Definition inv_set_size st : Prop :=
+  length st.(from_set) = length st.(collected_lightsigs) /\
+  length st.(from_set) = length st.(collected_sigs).
+
+Definition inv_conf_correct st : Prop :=
+  if st.(conf)
+  then length st.(from_set) = N - t0
+  else length st.(from_set) < N - t0.
+
+Definition inv_from_nodup st : Prop :=
+  NoDup st.(from_set).
+
+(* "NoDup nsigs" and "N - t0 <= (length nsigs)" should also hold 
+    even if the certificate is sent by a Byzantine node *)
+
+Definition inv_rlcerts st : Prop :=
+  forall v cs, In (v, cs) st.(received_lightcerts) -> 
+    combined_verify v cs.
+
+Definition inv_rcerts_mixin st : Prop :=
+  forall v nsigs, In (v, nsigs) st.(received_certs) -> 
+    certificate_valid v nsigs /\
+    (NoDup nsigs) /\ 
+    N - t0 <= (length nsigs).
+
+Definition inv_submit_mixin st : Prop :=
+  match st.(submitted_value) with
+  | Some v => 
+    v = value_bft st.(id) /\
+    light_signatures_valid v (zip_from_lsigs st) /\
+    certificate_valid v (zip_from_sigs st)
+  | None => st.(from_set) = nil
+  end.
+
+Definition inv_submit_none st : Prop :=
+  st.(submitted_value) = None -> st.(from_set) = nil.
+
+Fact inv_submit_mixin_break st : inv_submit_mixin st -> inv_submit_none st.
+Proof. unfold inv_submit_mixin, inv_submit_none. intros H E. now rewrite E in H. Qed.
+
+Definition buffer_nil_after_submit st : Prop :=
+  st.(submitted_value) -> st.(msg_buffer) = nil.
+
+Definition buffer_contains_submitmsg st : Prop :=
+  forall nmsg, In nmsg st.(msg_buffer) ->
+    match snd nmsg with SubmitMsg _ _ _ => True | _ => False end.
+
+Definition confirmed_then_submitted st : Prop :=
+  st.(conf) -> st.(submitted_value).
+
+(* l2h, sent *)
+
+Definition inv_submitted_broadcast psent st : Prop :=
+  forall v, st.(submitted_value) = Some v ->
+    let: src := st.(id) in
+    forall n, exists used, 
+      In (mkP src n (SubmitMsg v (light_sign v (lightkey_map src)) (sign v (key_map src))) used) psent.
+
+Definition inv_conf_lightconfmsg psent st : Prop :=
+  forall v, st.(submitted_value) = Some v ->
+    st.(conf) -> forall n,
+    exists used, In (mkP st.(id) n (LightConfirmMsg (v, lightsig_combine st.(collected_lightsigs))) used) psent.
+
+Definition inv_conf_confmsg psent st : Prop :=
+  forall v, st.(submitted_value) = Some v ->
+    st.(conf) -> lightcert_conflict_check st.(received_lightcerts) -> (* coinciding with control flow *)
+    forall n,
+      exists used, In (mkP st.(id) n (ConfirmMsg (v, zip_from_sigs st)) used) psent.
+
+(* l2h, recv *)
+
+Definition inv_nsigs_correct psent st : Prop :=
+  forall v, st.(submitted_value) = Some v ->
+    forall n lsig sig, 
+      In (n, lsig, sig) (zip_from_lsigs_sigs st) ->
+        In (mkP n st.(id) (SubmitMsg v lsig sig) true) psent.
+
+Definition inv_rlcerts_correct psent st : Prop :=
+  forall lc,
+    In lc st.(received_lightcerts) ->
+      exists src, In (mkP src st.(id) (LightConfirmMsg lc) true) psent.
+
+Definition inv_rcerts_correct psent st : Prop :=
+  forall c,
+    In c st.(received_certs) ->
+      exists src, In (mkP src st.(id) (ConfirmMsg c) true) psent.
+
+Definition inv_buffer_received psent st : Prop :=
+  forall nmsg, In nmsg st.(msg_buffer) ->
+    In (mkP (fst nmsg) st.(id) (snd nmsg) true) psent.
+
+(* h2l, sent *)
+
+Definition inv_submitmsg_correct p stmap : Prop :=
+  match p with
+  | mkP src dst (SubmitMsg v lsig sig) used =>
+    let: st := stmap src in
+    is_byz src = false ->
+      verify v sig src /\
+      light_verify v lsig src /\
+      st.(submitted_value) = Some v (* TODO why put some at LHS? *)
+  | _ => True
+  end.
+
+(* CHECK conjecture: only Byzantine messages require the history argument?
+  only non-Byz messages require the stmap argument? *)
+Definition inv_lightconfirmmsg_correct_nonbyz p stmap : Prop :=
+  match p with
+  | mkP src dst (LightConfirmMsg lc) used =>
+    let: st := stmap src in
+    is_byz src = false ->
+      st.(conf) /\ st.(submitted_value) = Some (fst lc) /\
+      snd lc = lightsig_combine st.(collected_lightsigs)
+  | _ => True
+  end.
+
+Definition inv_lightconfirmmsg_correct_byz p psent_history : Prop :=
+  match p with
+  | mkP src dst (LightConfirmMsg lc) used =>
+    is_byz src -> lcert_correct_threshold psent_history lc
+  | _ => True
+  end.
+
+Definition inv_confirmmsg_correct_nonbyz p stmap : Prop :=
+  match p with
+  | mkP src dst (ConfirmMsg c) used =>
+    let: st := stmap src in
+    is_byz src = false ->
+      st.(conf) /\ lightcert_conflict_check st.(received_lightcerts) (* this is new *)
+      /\ st.(submitted_value) = Some (fst c) /\
+      snd c = zip_from_sigs st
+  | _ => True
+  end.
+
+Definition inv_confirmmsg_correct_byz p psent_history : Prop :=
+  match p with
+  | mkP src dst (ConfirmMsg c) used =>
+    is_byz src -> cert_correct psent_history c
+  | _ => True
+  end.
+
+(* h2l, recv *)
+
+(* this is a rather non-trivial invariant since it depends on node state
+    and should be proved individually *)
+Definition inv_submitmsg_receive_ p st : Prop :=
+  match p.(msg) with
+  | SubmitMsg v lsig sig =>
+    if p.(consumed)
+    then
+      let: src := p.(src) in
+      let: dst := p.(dst) in
+      is_byz dst = false ->
+      match st.(submitted_value) with
+      | None => In (src, SubmitMsg v lsig sig) st.(msg_buffer)
+      | Some ov => 
+        (* the length condition may be more natural, but it would be hard to reason about 
+          without invariant 1; so replace it with the condition on conf *)
+        (* length st.(from_set) < N - t0 -> *)
+        st.(conf) = false ->
+        v = ov -> verify v sig src -> light_verify v lsig src ->
+          In src st.(from_set) (* this should be enough; TODO why no need to write zip_from_sigs? *)
+      end
+    else True
+  | _ => True
+  end.
+
+Definition inv_submitmsg_receive p stmap : Prop := inv_submitmsg_receive_ p (stmap p.(dst)).
+
+Definition inv_lightconfirmmsg_receive p stmap : Prop :=
+  match p with
+  | mkP src dst (LightConfirmMsg (v, cs)) true =>
+    let: st := stmap dst in
+    is_byz dst = false ->
+    combined_verify v cs -> In (v, cs) st.(received_lightcerts)
+  | _ => True
+  end.
+
+Definition inv_confirmmsg_receive p stmap : Prop :=
+  match p with
+  | mkP src dst (ConfirmMsg (v, nsigs)) true =>
+    let: st := stmap dst in
+    is_byz dst = false ->
+    certificate_valid v nsigs -> NoDup nsigs -> (N - t0 <= (length nsigs)) ->
+      In (v, nsigs) st.(received_certs)
+  | _ => True
+  end.
+
+(* persistence *)
+
+Definition submitted_value_persistent st st' : Prop :=
+  forall v, st.(submitted_value) = Some v -> st'.(submitted_value) = Some v.
+
+Definition conf_persistent st st' : Prop := st.(conf) -> st'.(conf).
+
+(* ideally, this would be used together with "buffer_nil_after_submit" *)
+Definition msg_buffer_nil_persistent st st' : Prop := 
+  st.(submitted_value) -> st.(msg_buffer) = nil -> st'.(msg_buffer) = nil.
+
+Definition msg_buffer_notnil_persistent st st' : Prop := 
+  st'.(submitted_value) = None -> 
+  forall nmsg, In nmsg st.(msg_buffer) -> In nmsg st'.(msg_buffer).
+
+(* the following will be useful in proving psent_mnt_sound *)
+Definition conf_from_set_persistent st st' : Prop := 
+  st.(conf) -> st.(from_set) = st'.(from_set).
+
+Definition conf_collected_lightsigs_persistent st st' : Prop := 
+  st.(conf) -> st.(collected_lightsigs) = st'.(collected_lightsigs).
+
+Definition conf_collected_sigs_persistent st st' : Prop := 
+  st.(conf) -> st.(collected_sigs) = st'.(collected_sigs).
+
+Definition from_set_persistent st st' : Prop :=
+  forall n, In n st.(from_set) -> In n st'.(from_set).
+
+Definition received_lightcerts_persistent st st' : Prop := 
+  forall lc, In lc st.(received_lightcerts) -> In lc st'.(received_lightcerts).
+
+Definition received_certs_persistent st st' : Prop := 
+  forall c, In c st.(received_certs) -> In c st'.(received_certs).
+
+Fact lightcert_conflict_check_persistent st st' (H : received_lightcerts_persistent st st') :
+  lightcert_conflict_check st.(received_lightcerts) ->
+  lightcert_conflict_check st'.(received_lightcerts).
+Proof.
+  intros Hb. rewrite lightcert_conflict_check_correct in Hb |- *. 
+  destruct Hb as (v1 & v2 & cs1 & cs2 & Hb). destruct_and? Hb.
+  exists v1, v2, cs1, cs2. hnf in H. intuition.
+Qed.
+
+Definition id_persistent st st' : Prop := st.(id) = st'.(id).
+
+Fact valid_cert_valid_sig v nsigs
+  (Hcert_valid : certificate_valid v nsigs) 
+  n sig (Hin : In (n, sig) nsigs) : sig = sign v (key_map n).
+Proof.
+  unfold certificate_valid in Hcert_valid.
+  rewrite -> Forall_forall in Hcert_valid.
+  now apply Hcert_valid, key_correct in Hin.
+Qed. 
+
+Fact valid_cert_sender_in v nsigs
+  (Hcert_valid : certificate_valid v nsigs) 
+  n (Hin : In n (map fst nsigs)) : In (n, sign v (key_map n)) nsigs.
+Proof.
+  apply in_map_iff in Hin.
+  destruct Hin as ((n', s) & Heq & ?).
+  simpl in Heq.
+  subst n'.
+  pose proof H as H'.
+  eapply valid_cert_valid_sig in H; eauto.
+  now subst s.
+Qed.
+
+Fact valid_cert_nodup_implies_sender_nodup v nsigs
+  (Hcert_valid : certificate_valid v nsigs) 
+  (Hcert_nodup : NoDup nsigs) : NoDup (map fst nsigs).
+Proof.
+  clear -Hcert_nodup Hcert_valid.
+  induction nsigs as [ | (n, sig) nsigs IH ].
+  - constructor.
+  - inversion_clear Hcert_nodup as [ | ? ? Hnotin Hcert_nodup' ].
+    apply Forall_cons_iff in Hcert_valid.
+    simpl in Hcert_valid.
+    destruct Hcert_valid as (Hveri & Hcert_valid).
+    rewrite <- key_correct in Hveri.
+    subst sig.
+    constructor.
+    + intros Hin.
+      now eapply valid_cert_sender_in in Hin; eauto.
+    + apply IH; intuition.
+Qed.
+
+Section Main_Proof.
+
+Set Implicit Arguments. (* anyway *)
+
+Tactic Notation "simpl_state" :=
+  simpl id in *; simpl conf in *; simpl submitted_value in *; simpl from_set in *;
+  simpl collected_lightsigs in *; simpl collected_sigs in *; simpl received_lightcerts in *; 
+  simpl received_certs in *; simpl msg_buffer in *.
+
+Create HintDb ABCinv.
+
+Tactic Notation "basic_solver" :=
+  try reflexivity; auto with ABCinv; try tauto; try eqsolve; try lia.
+
+Local Hint Resolve correct_sign_verify_ok correct_sign_verify_ok_light : ABCinv.
+
+Local Hint Resolve incl_sendout_l incl_sendout_r incl_sendout_app_l incl_sendout_app_r : ABCinv.
+
+Local Hint Resolve incl_nil_l : datatypes.
+
+Section State_Monotone_Proofs.
+
+Inductive state_mnt_type (st : State) : Type :=
+  | Msubmit : st.(submitted_value) = None -> state_mnt_type st
+  | Mconf : forall v, st.(submitted_value) = Some v ->
+    (* conf may be already true *) state_mnt_type st
+  | Mfrom_in : forall src v lsig sig, 
+    st.(submitted_value) = Some v ->
+    verify v sig src -> light_verify v lsig src ->
+    st.(conf) = false -> ~ In src st.(from_set) -> state_mnt_type st
+  | Mfrom_buffer : forall (src : Address) (v : Value) (lsig : LightSignature) (sig : Signature), 
+    st.(submitted_value) = None -> state_mnt_type st
+  | Mlcert : forall (src : Address) v cs,
+    combined_verify v cs -> state_mnt_type st
+  | Mcert : forall (src : Address) v nsigs,
+    NoDup nsigs -> (N - t0) <= length nsigs -> certificate_valid v nsigs -> 
+    state_mnt_type st
+(*   
+  | Mcheck : forall v, (* even the state will not change, it is still required for l2h proof *)
+    st.(submitted_value) = Some v ->
+    st.(conf) -> lightcert_conflict_check st.(received_lightcerts) ->
+    state_mnt_type st
+     *)
+.
+
+Global Arguments Mconf : clear implicits.
+Global Arguments Mfrom_in : clear implicits.
+Global Arguments Mlcert : clear implicits. 
+Global Arguments Mcert : clear implicits. 
+(* Global Arguments Mcheck : clear implicits.  *)
+
+Definition state_mnt (st : State) (s : state_mnt_type st) : State :=
+  match s with
+  | Msubmit _ _ =>
+    (st <| submitted_value := Some (value_bft st.(id)) |>
+        <| msg_buffer := nil |>)
+  | Mconf _ _ _=>
+    (st <| conf := true |>)
+  | Mfrom_in _ src _ lsig sig _ _ _ _ _ =>
+    (st <| from_set := src :: st.(from_set) |>
+        <| collected_lightsigs := lsig :: st.(collected_lightsigs) |> 
+        <| collected_sigs := sig :: st.(collected_sigs) |>)
+  | Mfrom_buffer _ src v lsig sig _ =>
+    (st <| msg_buffer := (src, SubmitMsg v lsig sig) :: st.(msg_buffer) |>)
+  | Mlcert _ _ v cs _ =>
+    (st <| received_lightcerts := (v, cs) :: st.(received_lightcerts) |>)
+  | Mcert _ _ v nsigs _ _ _ =>
+    (st <| received_certs := (v, nsigs) :: st.(received_certs) |>)
+  (* | Mcheck _ v _ _ _ =>
+    st *)
+  end.
+
+Definition confirmmsg_bcast st :=
+  match st.(submitted_value) with
+  | Some v => broadcast st.(id) (ConfirmMsg (v, zip_from_sigs st))
+  | None => nil
+  end.
+
+(* I guess in theory, there isn't a perfect solution;
+    either prove "inv_buffer_received" first (which means you would need another 2-3 proofs, 
+    one being induction), or have a ghost variable like this (and potentially complicate
+    other proofs). *) 
+(* the ghost variable "other_pkts" is really like opening a backdoor ... *)
+(* ... which greatly complicates the other proofs. I can no longer tolerate it *)
+(*
+Definition psent_effect (st : State) (s : state_mnt_type st) (n : Address) (psent : PacketSoup) (other_pkts : list Packet) : Prop :=
+  Eval unfold confirmmsg_bcast in
+  match s with
+  | Msubmit _ _ =>
+    let: n := st.(id) in
+    let: v := value_bft n in
+    let: pkts := broadcast n (SubmitMsg v (light_sign v (lightkey_map n)) (sign v (key_map n))) in
+    incl pkts psent
+  | Mconf _ v _ =>
+    (* let: pkts := broadcast st.(id) (LightConfirmMsg (v, lightsig_combine st.(collected_lightsigs))) in
+    incl pkts psent *)
+    (* HMM might be a trick *)
+    (let: pkts := broadcast st.(id) (LightConfirmMsg (v, lightsig_combine st.(collected_lightsigs))) in
+    incl pkts psent) /\
+    (lightcert_conflict_check st.(received_lightcerts) ->
+    incl (confirmmsg_bcast st) psent)
+  | Mfrom_in _ src v lsig sig _ _ _ _ _ =>
+    In (mkP src n (SubmitMsg v lsig sig) true) psent
+    \/ In (mkP src n (SubmitMsg v lsig sig) true) other_pkts (* ghost state? *)
+  | Mfrom_buffer _ src v lsig sig _ =>
+    In (mkP src n (SubmitMsg v lsig sig) true) psent
+  | Mlcert _ src v cs _ =>
+    (In (mkP src n (LightConfirmMsg (v, cs)) true) psent
+    \/ In (mkP src n (LightConfirmMsg (v, cs)) true) other_pkts) 
+    /\
+    (st.(conf) -> lightcert_conflict_check ((v, cs) :: st.(received_lightcerts)) ->
+    incl (confirmmsg_bcast st) psent)
+  | Mcert _ src v nsigs _ _ _ =>
+    In (mkP src n (ConfirmMsg (v, nsigs)) true) psent
+    \/ In (mkP src n (ConfirmMsg (v, nsigs)) true) other_pkts
+  (* | Mcheck _ v _ _ _ =>
+    let: pkts := broadcast st.(id) (ConfirmMsg (v, zip_from_sigs st)) in
+    incl pkts psent *)
+  end.
+*)
+Definition psent_effect (st : State) (s : state_mnt_type st) (n : Address) (psent : PacketSoup) : Prop :=
+  Eval unfold confirmmsg_bcast in
+  match s with
+  | Msubmit _ _ =>
+    let: n := st.(id) in
+    let: v := value_bft n in
+    let: pkts := broadcast n (SubmitMsg v (light_sign v (lightkey_map n)) (sign v (key_map n))) in
+    incl pkts psent
+  | Mconf _ v _ =>
+    (* let: pkts := broadcast st.(id) (LightConfirmMsg (v, lightsig_combine st.(collected_lightsigs))) in
+    incl pkts psent *)
+    (* HMM might be a trick *)
+    (let: pkts := broadcast st.(id) (LightConfirmMsg (v, lightsig_combine st.(collected_lightsigs))) in
+    incl pkts psent) /\
+    (lightcert_conflict_check st.(received_lightcerts) ->
+    incl (confirmmsg_bcast st) psent)
+  | Mfrom_in _ src v lsig sig _ _ _ _ _ =>
+    In (mkP src n (SubmitMsg v lsig sig) true) psent
+  | Mfrom_buffer _ src v lsig sig _ =>
+    In (mkP src n (SubmitMsg v lsig sig) true) psent
+  | Mlcert _ src v cs _ =>
+    In (mkP src n (LightConfirmMsg (v, cs)) true) psent
+    /\
+    (st.(conf) -> lightcert_conflict_check ((v, cs) :: st.(received_lightcerts)) ->
+    incl (confirmmsg_bcast st) psent)
+  | Mcert _ src v nsigs _ _ _ =>
+    In (mkP src n (ConfirmMsg (v, nsigs)) true) psent
+  end.
+
+Inductive state_mnt_type_list : State -> State -> Type :=
+  | MNTnil : forall st, state_mnt_type_list st st
+  | MNTcons : forall st (d : state_mnt_type st) st', 
+    state_mnt_type_list (state_mnt d) st' ->
+    state_mnt_type_list st st'.
+
+Fixpoint state_mnt_type_list_app [st st' st''] (l1 : state_mnt_type_list st st') (l2 : state_mnt_type_list st' st'') 
+  : state_mnt_type_list st st''.
+  destruct l1.
+  - exact l2.
+  - exact (MNTcons d (state_mnt_type_list_app _ _ _ l1 l2)).
+Defined.
+(*
+Fixpoint psent_effect_star (n : Address) (psent : PacketSoup) (other_pkts : list Packet) [st st'] (l : state_mnt_type_list st st') : Prop :=
+  match l with
+  | MNTnil _ => True
+  | MNTcons d l' =>
+    psent_effect d n psent other_pkts /\ psent_effect_star n psent other_pkts l' (* TODO setting implicit during definition? *)
+  end.
+*)
+Fixpoint psent_effect_star (n : Address) (psent : PacketSoup) [st st'] (l : state_mnt_type_list st st') : Prop :=
+  match l with
+  | MNTnil _ => True
+  | MNTcons d l' =>
+    psent_effect d n psent /\ psent_effect_star n psent l' (* TODO setting implicit during definition? *)
+  end.
+(*
+Lemma psent_effect_star_app n psent others st st' st'' (l1 : state_mnt_type_list st st') (l2 : state_mnt_type_list st' st'') :
+  psent_effect_star n psent others (state_mnt_type_list_app l1 l2) <-> 
+  psent_effect_star n psent others l1 /\ psent_effect_star n psent others l2.
+Proof. revert st'' l2. induction l1; intros; simpl; try tauto. rewrite IHl1. tauto. Qed.
+
+Lemma psent_effect_star_incl n psent psent' others others' st st' (l : state_mnt_type_list st st')
+  (H : psent_effect_star n psent others l) (Hincl : incl psent psent') (Hincl' : incl others others') :
+  psent_effect_star n psent' others' l.
+Proof. induction l; simpl in *; auto. destruct H. split; auto. destruct d; simpl in *; unfold incl in *; intuition. Qed.
+*)
+Lemma psent_effect_star_app n psent st st' st'' (l1 : state_mnt_type_list st st') (l2 : state_mnt_type_list st' st'') :
+  psent_effect_star n psent (state_mnt_type_list_app l1 l2) <-> 
+  psent_effect_star n psent l1 /\ psent_effect_star n psent l2.
+Proof. revert st'' l2. induction l1; intros; simpl; try tauto. rewrite IHl1. tauto. Qed.
+
+Lemma psent_effect_star_incl n psent psent' st st' (l : state_mnt_type_list st st')
+  (H : psent_effect_star n psent l) (Hincl : incl psent psent') :
+  psent_effect_star n psent' l.
+Proof. induction l; simpl in *; auto. destruct H. split; auto. destruct d; simpl in *; unfold incl in *; intuition. Qed.
+(* 
+(* false: stopping token *)
+Local Ltac state_analyze_select f x :=
+  match f with
+  | msg_buffer =>
+    match x with
+    | _ :: _ => uconstr:(Mfrom_buffer)
+    | _ => uconstr:(false)
+    end
+  | collected_sigs => uconstr:(Mfrom_in)
+  | received_lightcerts => uconstr:(Mlcert)
+  | received_certs => uconstr:(Mcert)
+  | _ => uconstr:(false)
+  end. 
+*)
+(* TODO eassumption is not stable ... mostly manual analysis below *)
+Ltac analyze_step ctor tac :=
+  unshelve eapply MNTcons; [ eapply ctor; tac | ]; simpl.
+(*
+Ltac state_analyze' st' :=
+  match st' with
+  | set ?f (fun _ => ?vv) ?st =>
+    let ctor := state_analyze_select f vv in
+    match ctor with
+    | false => idtac
+    | _ =>
+      state_analyze' st;
+      match goal with 
+      | |- state_mnt_type_list _ _ =>
+        unshelve eapply MNTcons; [ eapply ctor | ]; simpl
+      | _ => idtac
+      end
+    end
+  | _ => idtac
+  end.
+*)
+Ltac psent_effect_star_solver :=
+  simpl; autorewrite with psent; rewrite ! In_consume; simpl; try solve [ tauto | intuition | basic_solver ].
+
+(* TODO this seems not to work as intended *)
+Ltac state_invariants_pre_solver :=
+  try solve 
+    [ constructor; hnf; intros HH; hnf in HH |- *; intros; simpl in *; basic_solver; try (now isSome_rewrite)
+    | intros; try rewrite sendout0; autorewrite with psent; 
+      solve [ auto using In_consume_fwd_full' with ABCinv |
+        intuition (auto using In_consume_fwd_full' with ABCinv) ] (* for inv_buffer_received *) ].
+
+Ltac local_solver := split_and?; try solve [ intros; eqsolve | psent_effect_star_solver | state_invariants_pre_solver ].
+(*
+Ltac state_analyze :=
+  try rewrite sendout0;
+  match goal with
+  | |- exists (_ : state_mnt_type_list _ ?st'), _ =>
+    unshelve eexists; [ state_analyze' st'; try solve [ apply (MNTnil _) ] | ];
+    split_and?;
+    match goal with
+    | |- @psent_effect_star _ _ _ _ _ => psent_effect_star_solver
+    | _ => try solve [ basic_solver ]
+    end
+  end.
+*)
+Definition lift_point_to_edge {A : Type} (P : A -> Prop) : A -> A -> Prop :=
+  fun st st' => P st -> P st'.
+
+(* here no need to put too many things in *)
+Record node_state_invariants_pre st st' : Prop := {
+  _ : lift_point_to_edge inv_conf_correct st st';
+  (* _ : lift_point_to_edge confirmed_then_submitted st st'; *)
+}.
+(*
+Fact inv_conf_confmsg_incl psent psent' st (H : inv_conf_confmsg psent st)
+  (Hincl : incl psent psent') : inv_conf_confmsg psent' st.
+Proof. hnf in *. intros. saturate_assumptions!. destruct H. specialize (Hincl _ H). eauto. Qed.
+*)
+(* the conditions get complicated to accommodate the ghost variable *)
+(*
+Fact state_mnt_sound_pre_pre p (Hnonbyz : is_byz (dst p) = false) stf msf w w'
+  (Ef : procMsgWithCheck (w @ dst p) (src p) (msg p) = (stf, msf))
+  psent others (E0 : w' = mkW (upd (dst p) stf (localState w)) (sendout msf psent))
+  (*
+  (Hothers : match (w @ dst p).(submitted_value) with None => others = nil | _ => True end)
+  (Hin : In (receive_pkt p) psent \/ (match p.(msg) with SubmitMsg _ _ _ => In (receive_pkt p) others | _ => False end)) :
+  *)
+  (Hothers : match (w @ dst p).(submitted_value) with None => others = nil | _ => True end)
+  (Hin : In (receive_pkt p) psent \/ In (receive_pkt p) others) :
+  forall n, exists l : state_mnt_type_list (w @ n) (w' @ n),
+    psent_effect_star n (sentMsgs w') others l /\ node_state_invariants_pre (w @ n) (w' @ n).
+Proof with (try (now exists (MNTnil _))).
+  destruct p as [ src dst msg used ]. simpl_pkt. subst w'. simpl. intros n. unfold procMsgWithCheck in Ef.
+  unfold upd.
+  destruct (Address_eqdec _ _) as [ <- | Hneq ]...
+  destruct (procMsg _ _ _) as [ (st', ms) | ] eqn:E in Ef; simplify_eq...
+  destruct (w @ dst) as [ dst' conf ov from lsigs sigs rlcerts rcerts buffer ].
+  destruct msg as [ v ls s | (v, cs) | (v, nsigs) ]; simpl in E.
+  1-2: simplify_eq. (* pair inj *)
+  1: simpl in Hin.
+  - destruct ov as [ vthis | ].
+    + destruct (andb _ _) eqn:EE in E; try discriminate. 
+      unfold is_left in EE. rewrite ! andb_true_iff, sumbool_is_left in EE. destruct EE as ((-> & Everi) & Elveri).
+      destruct conf.
+      * simplify_eq. unshelve eexists. 1: analyze_step Mconf ltac:(idtac); try apply MNTnil; try reflexivity. 
+        simpl. destruct (lightcert_conflict_check _) in |- *; simpl.
+        all: local_solver.
+      * destruct (in_dec _ _ _) as [ | Hnotin ] in E; try discriminate. simplify_eq.
+        destruct (N - t0 <=? S (length from)) eqn:Eth; 
+          [ apply Nat.leb_le in Eth | apply Nat.leb_nle in Eth ].
+        all: unshelve eexists; [ analyze_step Mfrom_in ltac:(try eassumption); auto | ]; try apply MNTnil.
+        1: analyze_step Mconf ltac:(idtac); auto. 1: apply MNTnil.
+        all: simpl. 1: destruct (lightcert_conflict_check _) in |- *; simpl.
+        all: local_solver.
+    + simplify_eq. simpl. unshelve eexists. 1: analyze_step Mfrom_buffer ltac:(idtac); try apply MNTnil; try reflexivity.
+      (* since here is for buffer, need to make sure that others = nil, so we need Hothers *)
+      simpl. simpl in Hothers. subst others. simpl in Hin. local_solver.
+  - destruct (combined_verify _ _) eqn:EE in E; try discriminate.
+    simplify_eq. unshelve eexists. 1: analyze_step Mlcert ltac:(idtac); try apply MNTnil; try reflexivity.
+    1: apply src. 1: auto. (* need to manually instantiate src here *)
+    simpl. unfold zip_from_sigs. simpl. rewrite app_nil_r.
+    destruct ov in |- *; [ destruct (andb _ _) eqn:EE0 in |- *; 
+      [ rewrite andb_true_iff in EE0 | rewrite andb_false_iff in EE0 ]; destruct EE0; try is_true_rewrite | ]; simpl.
+    all: local_solver.
+    (* ... *)
+    + (* TODO automation is so weak???? *) now setoid_rewrite H.
+    + auto with datatypes.
+  - destruct (andb _ _) eqn:EE in E; try discriminate.
+    unfold is_left in EE. rewrite ! andb_true_iff, ! sumbool_is_left, Nat.leb_le in EE. destruct_and? EE.
+    simplify_eq. unshelve eexists. 1: analyze_step Mcert ltac:(idtac); try apply MNTnil; try reflexivity.
+    1: apply src. all: auto. (* need to manually instantiate src here *)
+    simpl. local_solver.
+Qed.
+
+Fact state_mnt_sound_pre q (Hq_ : forall n t, q <> Intern n t) 
+  w w' (Hstep : system_step q w w') :
+  forall n, exists l : state_mnt_type_list (w @ n) (w' @ n),
+    psent_effect_star n (sentMsgs w') nil l /\ node_state_invariants_pre (w @ n) (w' @ n).
+    (* /\ (id (w @ n) = n (* ! *) -> is_byz n = false -> inv_buffer_received (sentMsgs w) (w @ n) -> 
+      inv_buffer_received (sentMsgs w') (w' @ n)). *)
+Proof with (try (now exists (MNTnil _))).
+  unfold inv_buffer_received.
+  inversion_step' Hstep; clear Hstep; intros... 
+  2: exfalso; eapply Hq_; reflexivity.
+  pose proof (@state_mnt_sound_pre_pre (mkP src dst msg used) Hnonbyz stf msf
+    w _ Ef (consume (mkP src dst msg used) (sentMsgs w)) nil eq_refl) as H.
+  simpl in H. apply H. now destruct (submitted_value _) in |- *. rewrite In_consume. auto.
+Qed.
+
+Definition buffer_augment n buf :=
+  map (fun nmsg => mkP (fst nmsg) n (snd nmsg) true) buf.
+
+Fact state_mnt_sound q w w' (Hstep : system_step q w w') :
+  forall n, exists l : state_mnt_type_list (w @ n) (w' @ n),
+    psent_effect_star n (sentMsgs w') 
+      (match q with Intern _ _ => buffer_augment n (w @ n).(msg_buffer) | _ => nil end) l /\ 
+    node_state_invariants_pre (w @ n) (w' @ n).
+    (* /\ (id (w @ n) = n (* ! *) -> is_byz n = false -> inv_buffer_received (sentMsgs w) (w @ n) -> 
+      inv_buffer_received (sentMsgs w') (w' @ n)). *)
+(* Proof with (try solve [ exists (MNTnil _); simpl; split_and?; local_solver ]). *)
+Proof with (try (now exists (MNTnil _))).
+  unfold inv_buffer_received.
+  destruct q as [ | | n0 t | ]. 1,2,4: eapply state_mnt_sound_pre; try eassumption; auto.
+  inversion_step' Hstep; clear Hstep; intros; try discriminate.
+  revert Hq. intros [= ->].
+  unfold upd.
+  destruct (Address_eqdec _ _) as [ <- | Hneq ]...
+  destruct t1, (w @ n) as [ n' conf ov from lsigs sigs rlcerts rcerts buffer ].
+  simpl in E. simpl.
+  destruct ov. 1: simplify_eq...
+  destruct (fold_right _ _ _) as (st_, ps_) eqn:Efr in E. simplify_eq.
+  (* this is great *)
+  change (set _ _ (set _ _ _)) with (Node n' conf (Some (value_bft n')) from lsigs sigs rlcerts rcerts nil) in Efr.
+  remember (Node _ _ _ _ _ _ _ _ _) as stt eqn:Es in Efr.
+  match goal with |- exists (_ : _), (psent_effect_star _ ?pp ?ot _) /\ _ =>
+    assert (exists l : state_mnt_type_list stt st', psent_effect_star n pp ot l /\ node_state_invariants_pre stt st') as Hgoal end.
+  all: subst stt.
+  (* time to do induction *)
+  { revert st' ps_ Efr. induction buffer as [ | (src, msg) buffer IH ]; intros; simpl in Efr.
+    - simplify_eq...
+    - simpl.
+      destruct (procMsgWithCheck _ _ _) as (sta, psa) eqn:E0 in Efr.
+      destruct (fold_right _ _ _) as (stb, psb) eqn:E1 in Efr. rewrite E1 in E0. simpl in E0, Efr. 
+      revert Efr. intros [= <- <-].
+      saturate_assumptions!. destruct IH as (l & Ha & HH).
+      (* use persistence here *)
+      pick submitted_value_persistent as_ Hv by_ (destruct HH). simpl in Hv. specialize (Hv _ eq_refl).
+      (* use the previous lemma *)
+      pose proof (@state_mnt_sound_pre_pre (mkP src n msg true) Hnonbyz sta psa
+        (mkW (upd n stb (localState w)) (sentMsgs w)) _ ltac:(simpl; rewrite upd_refl; assumption)
+        (sentMsgs w) (mkP src n msg true :: nil) eq_refl ltac:(simpl; rewrite upd_refl, Hv; auto) ltac:(simpl; auto) n) as Hgoal.
+      simpl in Hgoal. rewrite ! upd_refl in Hgoal. destruct Hgoal as (l0 & Ha0 & HH0).
+      exists (state_mnt_type_list_app l l0). 
+      rewrite psent_effect_star_app. split; [ split; [ eapply psent_effect_star_incl; try apply Ha | eapply psent_effect_star_incl; try apply Ha0 ] | ].
+      1-4: hnf; intros ?; autorewrite with psent; simpl; tauto.
+      pick submitted_value_persistent as_ Hv0 by_ (destruct HH0). specialize (Hv0 _ Hv).
+      destruct HH, HH0. hnf in *. state_invariants_pre_solver. }
+  destruct Hgoal as (l & Ha & HH).
+  unshelve eexists. 1: analyze_step Msubmit ltac:(idtac); try apply MNTnil; try reflexivity. 1: apply l.
+  simpl; local_solver.
+  (* TODO still need some cleaning! *)
+  destruct HH as [ HH1 HH2 HH3 ]. hnf in *. constructor; auto; try discriminate. 
+  hnf; intros; hnf in *; intros. apply HH2; auto. now hnf.
+Qed.
+*)
+Definition lift_node_inv (P : PacketSoup -> State -> Prop) : World -> Prop :=
+  fun w => forall n, is_byz n = false -> P (sentMsgs w) (w @ n).
+
+(* FIXME: 
+
+  This poses a problem about proving invariants: sometimes several invariants need 
+  to be grouped together to prove, otherwise we need several proofs for each invariant. 
+  However, proving the grouped invariants will make the invariants "harder" to use, 
+  since we need to satisfy all the invariants at the same time to use only one of them. 
+
+  One way to work around is to use the notion of reachable worlds. By proving the 
+  grouped invariant always holds on reachable worlds, one can then "split" the grouped
+  invariants. However, this is also not perfect since this requires the world to be 
+  actually reachable. When we do not know that condition or that condition has to be 
+  proved separately (e.g., by simulation), things will again get complicated. 
+  This can happen when there is (mutual recursion) between transitions; see ABC for 
+  an example. 
+
+  Another potentially better way is to have finer-grained dependency. For example, if
+  invariant B depends on A, while A only depends on itself, then the proof goal can be 
+  written as:
+
+  (A -> A') /\ (A /\ B -> B')
+
+  This nevertheless requires some repeating in the proof goal and some intricate 
+  manipulation of the proof context (e.g., the hypotheses are different for each subgoal), 
+  but should be able to resolve the problem above. 
+
+  Maybe in the future, we can consider develop some way to state that dependency easily 
+  and manage the proof context. 
+*)
+Fact inv_buffer_received_only_pre q (Hq_ : forall n t, q <> Intern n t) 
+  w w' (Hstep : system_step q w w') 
+  (H : forall n, (w @ n).(id) = n /\ (is_byz n = false -> inv_buffer_received (sentMsgs w) (w @ n))
+    /\ ((w @ n).(submitted_value) -> (w @ n).(msg_buffer) = nil)) :
+  (* we need all four of them for the induction proof *)
+  forall n, (w' @ n).(id) = n /\ (is_byz n = false -> inv_buffer_received (sentMsgs w') (w' @ n))
+    /\ ((w' @ n).(submitted_value) -> (w' @ n).(msg_buffer) = nil)
+    /\ submitted_value_persistent (w @ n) (w' @ n).
+Proof with (intros; rewrite ?sendout0; try (rewrite In_sendout; right); eauto using In_consume_fwd_full').
+  (* destruct H as (Hcoh & Hrcv).
+  unfold id_coh, lift_node_inv.
+  enough (forall n, id (w' @ n) = n /\ (is_byz n = false → inv_buffer_received (sentMsgs w') (w' @ n))) as H.
+  { split; intros n; specialize (H n); destruct H; saturate_assumptions; auto. }
+  intros n. specialize (Hrcv n). *)
+  intros n. specialize (H n). destruct H as (Hcoh & Hrcv & Hs).
+  unfold inv_buffer_received, submitted_value_persistent in *.
+  inversion_step' Hstep; clear Hstep; auto.
+  3:{ split_and?; auto. intros. rewrite In_sendout1. right. eapply Hrcv; eauto. }
+  2: exfalso; eapply Hq_; reflexivity.
+  unfold upd.
+  destruct (Address_eqdec _ _) as [ <- | Hneq ].
+  2: split_and?; auto...
+  destruct (procMsg _ _ _) as [ (st', ms) | ] eqn:E in Ef; simplify_eq.
+  2: split_and?; auto...
+  (* get stf first *)
+  destruct (w @ dst) as [ dst' conf ov from lsigs sigs rlcerts rcerts buffer ] eqn: Est. simpl_state. subst dst'.
+  destruct msg as [ v ls s | (v, cs) | (v, nsigs) ]; simpl in E; simplify_eq. (* pair inj *)
+  - destruct ov as [ vthis | ].
+    + destruct (andb _ _) eqn:EE, conf in E; try discriminate; simplify_eq; simpl.
+      1: split_and?; auto...
+      destruct (in_dec _ _ _) as [ | Hnotin ] in E; try discriminate. simplify_eq. simpl.
+      split_and?; auto...
+    + simplify_eq. simpl. split_and?; auto; try discriminate. 
+      intros ?? [ <- | Hin ]; simpl... rewrite In_consume. tauto.
+  - destruct (combined_verify _ _) eqn:EE in E; try discriminate.
+    simplify_eq. split_and?; auto...
+  - destruct (andb _ _) eqn:EE in E; try discriminate.
+    simplify_eq. split_and?; auto...
+Qed.
+
+Fact inv_buffer_received_only q w w' (Hstep : system_step q w w') 
+  (H : forall n, (w @ n).(id) = n /\ (is_byz n = false -> inv_buffer_received (sentMsgs w) (w @ n))
+    /\ ((w @ n).(submitted_value) -> (w @ n).(msg_buffer) = nil)) :
+  forall n, (w' @ n).(id) = n /\ (is_byz n = false -> inv_buffer_received (sentMsgs w') (w' @ n))
+    /\ ((w' @ n).(submitted_value) -> (w' @ n).(msg_buffer) = nil)
+    /\ submitted_value_persistent (w @ n) (w' @ n).
+Proof.
+  destruct q as [ | | n t | ]. 
+  1,2,4: eapply inv_buffer_received_only_pre; try eassumption; auto.
+  unfold inv_buffer_received, submitted_value_persistent in *. intros n0.  
+  inversion_step' Hstep; intros; try discriminate.
+  revert Hq. intros [= <-]. destruct t1. 
+  unfold upd.
+  destruct (Address_eqdec _ _) as [ <- | Hneq ].
+  2: split_and?; auto; try apply H; intros; rewrite In_sendout; right; now apply H.
+  pose proof (proj1 (proj2 (H n)) Hnonbyz) as Hrcv. (* dealing with the in-out id issue, instantiate one for n *)
+  pose proof (fun n => proj1 (H n)) as Hcoh. pose proof (proj2 (proj2 (H n))) as Hs.
+  destruct_localState w n as_ [ ? conf ov from lsigs sigs rlcerts rcerts buffer ] eqn_ Est. simpl_state.
+  simpl in E.
+  destruct ov as [ v | ].
+  1: simplify_eq; simpl; split_and?; auto; intros; rewrite sendout0; now apply Hrcv.  
+  destruct (fold_right _ _ _) as (st_, ps_) eqn:Efr in E. simplify_eq.
+  change (set _ _ (set _ _ _)) with (Node n conf (Some (value_bft n)) from lsigs sigs rlcerts rcerts nil) in Efr. (* the extensionality is great *)
+  (* these are what we need to maintain in the induction proof *)
+  enough (id st' = n /\ st'.(msg_buffer) = nil /\ st'.(submitted_value)) as (<- & -> & _).
+  1: simpl; split_and?; auto; try discriminate; try contradiction.
+  (* time to do induction *)
+  clear Hstep Est Hs. revert st' ps_ Efr.
+  induction buffer as [ | (src, msg) buffer IH ]; intros; simpl in Efr.
+  - now simplify_eq.
+  - destruct (procMsgWithCheck _ _ _) as (sta, psa) eqn:E0 in Efr.
+    destruct (fold_right _ _ _) as (stb, psb) eqn:E1 in Efr. rewrite E1 in E0. simpl in E0, Efr. 
+    revert Efr. intros [= <- <-].
+    simpl in Hrcv. specialize (IH (fun a H => Hrcv a (or_intror H))).
+    saturate_assumptions! in_ IH. destruct IH as (Hidb & Hsb & Hvv).
+    (* use the previous lemma *)
+    specialize (Hrcv _ (or_introl eq_refl)). simpl in Hrcv.
+    epose proof (DeliverStep (Deliver (mkP src n msg true)) (mkW (upd n stb (localState w)) (sentMsgs w))
+      _ _ eq_refl Hrcv Hnonbyz ?[Goalq]).
+    [Goalq]: simpl; rewrite upd_refl, E0; reflexivity.
+    eapply inv_buffer_received_only_pre with (n:=n) in H0; auto.
+    2:{ simpl. intros. unfold upd. destruct (Address_eqdec _ _) as [ <- | Hneq ]; auto.
+      split_and?; auto. unfold inv_buffer_received. rewrite Hsb. simpl. contradiction. }
+    simpl in H0. rewrite !upd_refl in H0. destruct H0 as (? & _ & Hq1 & Hq2).
+    hnf in Hq2. destruct (stb.(submitted_value)) eqn:Ea; try discriminate. specialize (Hq2 _ eq_refl).
+    isSome_rewrite; auto.
+Qed.
+
+Definition lift_state_inv (P : State -> Prop) : World -> Prop := fun w => forall n, P (w @ n).
+
+Fact inv_buffer_received_only_reformat : always_holds
+  (fun w => id_coh w /\ lift_node_inv inv_buffer_received w /\ lift_state_inv buffer_nil_after_submit w).
+Proof.
+  apply grounded_invariant_always_holds. hnf; split.
+  1: split_and?; hnf; intros; hnf in *; intros; try reflexivity; try contradiction.
+  intros ??? (H1 & H2 & H3) Hstep. 
+  split_and?; intros n; eapply inv_buffer_received_only with (n:=n) in Hstep; try (intros; split_and?; hypothesis).
+  all: tauto.
+Qed.
+
+Fact id_coh_always_holds : always_holds id_coh.
+Proof. always_holds_decompose inv_buffer_received_only_reformat. Qed.
+
+(* HMM just proving always_hold may also be not satisfactory, since this is actually weaker 
+    than being an invariant ... this issue may come out in some other proofs that depend
+    on these invariants (e.g., proofs using id_coh) *)
+Fact inv_buffer_received_always_holds : always_holds (lift_node_inv inv_buffer_received).
+Proof. always_holds_decompose inv_buffer_received_only_reformat. Qed.
+
+Fact buffer_nil_after_submit_holds : always_holds (lift_state_inv buffer_nil_after_submit).
+Proof. always_holds_decompose inv_buffer_received_only_reformat. Qed.
+
+Fact state_mnt_sound_pre_pre q (Hq_ : forall n t, q <> Intern n t) 
+  w w' (Hstep : system_step q w w') :
+  forall n, exists l : state_mnt_type_list (w @ n) (w' @ n),
+    psent_effect_star n (sentMsgs w') l /\ node_state_invariants_pre (w @ n) (w' @ n)
+    (* this is not persistence! so need to prove here *)
+    /\ (w @ n).(submitted_value) = (w' @ n).(submitted_value).
+Proof with (try (now exists (MNTnil _))).
+  inversion_step' Hstep; clear Hstep; intros... 
+  2: exfalso; eapply Hq_; reflexivity.
+  unfold upd.
+  destruct (Address_eqdec _ _) as [ <- | Hneq ]...
+  destruct (procMsg _ _ _) as [ (st', ms) | ] eqn:E in Ef; simplify_eq...
+  destruct (w @ dst) as [ dst' conf ov from lsigs sigs rlcerts rcerts buffer ].
+  destruct msg as [ v ls s | (v, cs) | (v, nsigs) ]; simpl in E; simplify_eq. (* pair inj *)
+  - destruct ov as [ vthis | ].
+    + destruct (andb _ _) eqn:EE in E; try discriminate. 
+      unfold is_left in EE. rewrite ! andb_true_iff, sumbool_is_left in EE. destruct EE as ((-> & Everi) & Elveri).
+      destruct conf.
+      * simplify_eq. unshelve eexists. 1: analyze_step Mconf ltac:(idtac); try apply MNTnil; try reflexivity. 
+        simpl. destruct (lightcert_conflict_check _) in |- *; simpl.
+        all: local_solver.
+      * destruct (in_dec _ _ _) as [ | Hnotin ] in E; try discriminate. simplify_eq.
+        destruct (N - t0 <=? S (length from)) eqn:Eth; 
+          [ apply Nat.leb_le in Eth | apply Nat.leb_nle in Eth ].
+        all: unshelve eexists; [ analyze_step Mfrom_in ltac:(try eassumption); auto | ]; try apply MNTnil.
+        1: analyze_step Mconf ltac:(idtac); auto. 1: apply MNTnil.
+        all: simpl. 1: destruct (lightcert_conflict_check _) in |- *; simpl.
+        all: local_solver.
+    + simplify_eq. simpl. unshelve eexists. 1: analyze_step Mfrom_buffer ltac:(idtac); try apply MNTnil; try reflexivity.
+      (* since here is for buffer, need to make sure that others = nil, so we need Hothers *)
+      (* simpl. simpl in Hothers. subst others. simpl in Hin. local_solver. *)
+      simpl. local_solver.
+  - destruct (combined_verify _ _) eqn:EE in E; try discriminate.
+    simplify_eq. unshelve eexists. 1: analyze_step Mlcert ltac:(idtac); try apply MNTnil; try reflexivity.
+    1: apply src. 1: auto. (* need to manually instantiate src here *)
+    simpl. unfold zip_from_sigs. simpl. rewrite app_nil_r.
+    destruct ov in |- *; [ destruct (andb _ _) eqn:EE0 in |- *; 
+      [ rewrite andb_true_iff in EE0 | rewrite andb_false_iff in EE0 ]; destruct EE0; try is_true_rewrite | ]; simpl.
+    all: local_solver.
+    (* ... *)
+    + (* TODO automation is so weak???? *) now setoid_rewrite H.
+    + auto with datatypes.
+  - destruct (andb _ _) eqn:EE in E; try discriminate.
+    unfold is_left in EE. rewrite ! andb_true_iff, ! sumbool_is_left, Nat.leb_le in EE. destruct_and? EE.
+    simplify_eq. unshelve eexists. 1: analyze_step Mcert ltac:(idtac); try apply MNTnil; try reflexivity.
+    1: apply src. all: auto. (* need to manually instantiate src here *)
+    simpl. local_solver.
+Qed.
+(*
+Fact state_mnt_sound_pre q (Hq_ : forall n t, q <> Intern n t) 
+  w w' (Hstep : system_step q w w') :
+  forall n, exists l : state_mnt_type_list (w @ n) (w' @ n),
+    psent_effect_star n (sentMsgs w') nil l /\ node_state_invariants_pre (w @ n) (w' @ n).
+    (* /\ (id (w @ n) = n (* ! *) -> is_byz n = false -> inv_buffer_received (sentMsgs w) (w @ n) -> 
+      inv_buffer_received (sentMsgs w') (w' @ n)). *)
+Proof with (try (now exists (MNTnil _))).
+  unfold inv_buffer_received.
+  inversion_step' Hstep; clear Hstep; intros... 
+  2: exfalso; eapply Hq_; reflexivity.
+  pose proof (@state_mnt_sound_pre_pre (mkP src dst msg used) Hnonbyz stf msf
+    w _ Ef (consume (mkP src dst msg used) (sentMsgs w)) nil eq_refl) as H.
+  simpl in H. apply H. now destruct (submitted_value _) in |- *. rewrite In_consume. auto.
+Qed.
+
+Definition buffer_augment n buf :=
+  map (fun nmsg => mkP (fst nmsg) n (snd nmsg) true) buf.
+*)
+
+(* HMM one inconvenience of having reachable here is that some lemmas become weaker, 
+    as they depend on the decomposition here so they have to assume reachable (i.e., persistent_invariants),
+    which is though not required to prove them directly *)
+Fact state_mnt_sound q w w' (Hstep : system_step q w w') (Hw : reachable w) :
+  forall n, exists l : state_mnt_type_list (w @ n) (w' @ n),
+    psent_effect_star n (sentMsgs w') l /\ node_state_invariants_pre (w @ n) (w' @ n).
+    (* /\ (id (w @ n) = n (* ! *) -> is_byz n = false -> inv_buffer_received (sentMsgs w) (w @ n) -> 
+      inv_buffer_received (sentMsgs w') (w' @ n)). *)
+(* Proof with (try solve [ exists (MNTnil _); simpl; split_and?; local_solver ]). *)
+Proof with (try (now exists (MNTnil _))).
+  destruct q as [ | | n t | ]. 
+  1,2,4: intros n; eapply state_mnt_sound_pre_pre with (n:=n) in Hstep; try eassumption; auto;
+    destruct Hstep as (? & ? & ? & ?); eauto.
+  intros n0.
+  inversion_step' Hstep; clear Hstep; intros; try discriminate.
+  revert Hq. intros [= <-]. destruct t1.
+  unfold upd.
+  destruct (Address_eqdec _ _) as [ <- | Hneq ]...
+  pose proof (id_coh_always_holds Hw) as Hcoh.
+  pose proof (inv_buffer_received_always_holds Hw Hnonbyz) as Hrcv. hnf in Hrcv. 
+  destruct_localState w n as_ [ ? conf ov from lsigs sigs rlcerts rcerts buffer ] eqn_ Est. simpl_state.
+  simpl in E.
+  destruct ov. 1: simplify_eq...
+  destruct (fold_right _ _ _) as (st_, ps_) eqn:Efr in E. simplify_eq.
+  change (set _ _ (set _ _ _)) with (Node n conf (Some (value_bft n)) from lsigs sigs rlcerts rcerts nil) in Efr.
+  remember (Node _ _ _ _ _ _ _ _ _) as stt eqn:Es in Efr.
+  (* time to do induction *)
+  match goal with |- exists (_ : _), (psent_effect_star _ ?pp _) /\ _ =>
+    assert (exists l : state_mnt_type_list stt st', psent_effect_star n pp l /\ node_state_invariants_pre stt st') as Hgoal end.
+  all: subst stt.
+  { clear Est. revert st' ps_ Efr. induction buffer as [ | (src, msg) buffer IH ]; intros; simpl in Efr.
+    - simplify_eq...
+    - simpl.
+      destruct (procMsgWithCheck _ _ _) as (sta, psa) eqn:E0 in Efr.
+      destruct (fold_right _ _ _) as (stb, psb) eqn:E1 in Efr. rewrite E1 in E0. simpl in E0, Efr. 
+      revert Efr. intros [= <- <-].
+      simpl in Hrcv. specialize (IH (fun a H => Hrcv a (or_intror H))).
+      saturate_assumptions! in_ IH. destruct IH as (l & Ha & HH).
+      (* use the previous lemma *)
+      specialize (Hrcv _ (or_introl eq_refl)). simpl in Hrcv.
+      epose proof (DeliverStep (Deliver (mkP src n msg true)) (mkW (upd n stb (localState w)) (sentMsgs w))
+        _ _ eq_refl Hrcv Hnonbyz ?[Goalq]) as H.
+      [Goalq]: simpl; rewrite upd_refl, E0; reflexivity.
+      eapply state_mnt_sound_pre_pre with (n:=n) in H; auto. 
+      simpl_world. rewrite !upd_refl in H. destruct H as (l0 & Ha0 & HH0 & _).
+      exists (state_mnt_type_list_app l l0). 
+      rewrite psent_effect_star_app. split. 1: split; [ eapply psent_effect_star_incl; try apply Ha | eapply psent_effect_star_incl; try apply Ha0 ].
+      1-2: hnf; intros ?; autorewrite with psent; rewrite ?In_consume; simpl; try tauto.
+      1: naive_solver. (* interesting case; depend on Hrcv *)
+      destruct HH, HH0. hnf in *. state_invariants_pre_solver. }
+  destruct Hgoal as (l & Ha & HH).
+  unshelve eexists. 1: analyze_step Msubmit ltac:(idtac); try apply MNTnil; try reflexivity. 1: apply l.
+  simpl; local_solver.
+  (* TODO still need some cleaning! *)
+  destruct HH. hnf in *. constructor; auto.
+Qed.
+
+Record node_persistent_invariants st st' : Prop := {
+  _ : submitted_value_persistent st st';
+  _ : conf_persistent st st';
+  _ : id_persistent st st';
+  _ : msg_buffer_nil_persistent st st';
+  _ : conf_from_set_persistent st st';
+  _ : conf_collected_lightsigs_persistent st st';
+  _ : conf_collected_sigs_persistent st st';
+  _ : received_lightcerts_persistent st st';
+  _ : received_certs_persistent st st';
+  _ : from_set_persistent st st';
+  _ : msg_buffer_notnil_persistent st st';
+}.
+
+Record node_state_invariants_pre' st st' : Prop := {
+  _ : lift_point_to_edge inv_from_nodup st st';
+  _ : lift_point_to_edge inv_rlcerts st st';
+  _ : lift_point_to_edge inv_rcerts_mixin st st';
+  _ : lift_point_to_edge inv_submit_mixin st st';
+  _ : lift_point_to_edge buffer_nil_after_submit st st';
+  _ : lift_point_to_edge buffer_contains_submitmsg st st';
+  _ : lift_point_to_edge confirmed_then_submitted st st';
+}.
+
+(* FIXME: the meta things about persistence can be reused? *)
+#[export] Instance Transitive_node_persistent_invariants : Transitive node_persistent_invariants.
+Proof.
+  hnf. intros ??? H H0. destruct H, H0. constructor.
+  all: hnf; intuition.
+  1: congruence.
+  all: hnf in *.
+  all: try solve [ is_true_rewrite; saturate_assumptions; congruence; auto ].
+  - match goal with H : isSome ?a = true |- _ => destruct a eqn:EE; try discriminate end. 
+    saturate_assumptions!. isSome_rewrite. auto.
+  - destruct (submitted_value y); isSome_rewrite; try intuition.
+    saturate_assumptions!. congruence.
+Qed.
+
+Fact persistent_invariants_pre_pre st (d : state_mnt_type st) :
+  node_persistent_invariants st (state_mnt d) /\ node_state_invariants_pre' st (state_mnt d).
+Proof.
+  split_and?; constructor.
+  all: match goal with |- lift_point_to_edge ?def _ _ => unfold def | _ => idtac end; hnf.
+  all: intros; destruct d; subst; simpl in *; eauto;
+    try solve [ hypothesis | congruence | constructor; auto | isSome_rewrite; auto; discriminate | naive_solver ].
+  all: try match_option_rewrite; unfold zip_from_lsigs, zip_from_sigs; simpl.
+  - rewrite H. simpl. split_and?; hnf; auto with core.
+  - destruct_and? H. split_and?; hnf; auto with core.
+Qed.
+
+(* FIXME: this is reusable? *)
+(* FIXME: this name is misleading ... since it contains two things *)
+Fact persistent_invariants_pre st st' (l : state_mnt_type_list st st') :
+  node_persistent_invariants st st' /\ node_state_invariants_pre' st st'.
+Proof.
+  induction l.
+  - split_and?; constructor. all: hnf; auto.
+  - destruct_and? IHl.
+    pose proof (persistent_invariants_pre_pre d) as HH. destruct_and? HH.
+    split. 1: etransitivity; eauto.
+    do 2 (match goal with H : node_state_invariants_pre' _ _ |- _ => destruct H end).
+    constructor; hnf in *; auto.
+Qed.
+
+(* TODO is this wrapper actually useful? *)
+Definition lift_state_pair_inv (P : State -> State -> Prop) : World -> World -> Prop :=
+  fun w w' => forall n, P (w @ n) (w' @ n).
+
+Fact persistent_invariants q w w' (Hstep : system_step q w w') (Hw : reachable w) :
+  lift_state_pair_inv node_persistent_invariants w w'.
+Proof.
+  intros n.
+  eapply state_mnt_sound with (n:=n) in Hstep; auto.
+  destruct Hstep as (l & _).
+  eapply persistent_invariants_pre; eauto.
+Qed.
+
+Fact persistent_invariants_trace [w l] (Htrace : system_trace w l) (Hw : reachable w) :
+  lift_state_pair_inv node_persistent_invariants w (final_world w l).
+Proof.
+  revert w Hw Htrace. induction l as [ | (q, w') l' IH ]; simpl; intros.
+  - rewrite final_world_nil. hnf. intros ?. constructor; hnf; auto.
+  - pose proof (ReachableStep (proj1 Htrace) Hw) as Hw'.
+    rewrite final_world_cons. destruct Htrace as (Hstep%persistent_invariants & Htrace); auto.
+    saturate_assumptions! in_ IH. hnf in IH, Hstep |- *. intros n. specialize (Hstep n). specialize (IH n).
+    etransitivity; eauto.
+Qed. 
+
+Record node_state_invariants st : Prop := {
+  _ : inv_conf_correct st;
+
+  _ : confirmed_then_submitted st;
+  _ : inv_from_nodup st;
+  _ : inv_rlcerts st;
+  _ : inv_rcerts_mixin st;
+  _ : inv_submit_mixin st;
+  _ : buffer_nil_after_submit st;
+  _ : buffer_contains_submitmsg st;
+}.
+
+Fact state_invariants : always_holds (lift_state_inv node_state_invariants).
+Proof.
+  intros w Hw. induction Hw as [ | q w w' Hstep Hw H ]; auto.
+  - (* TODO streamline the proof here? *)
+    unfold initWorld, initState, Init.
+    hnf. intros n. constructor; simpl; hnf; simpl; try solve [ discriminate | contradiction | constructor; auto | lia | auto ].
+    pose proof t0_lt_N. lia.
+  - hnf. intros n. specialize (H n).
+    pose proof (state_mnt_sound Hstep Hw n) as (l & _ & Hinv_pre).
+    pose proof (persistent_invariants_pre l) as (_ & HH). 
+    destruct H, Hinv_pre, HH. unfold lift_point_to_edge in *. constructor; auto.
+Qed.
+
+End State_Monotone_Proofs.
+
+Section Forward.
+
+Record node_psent_l2h_invariants psent st : Prop := {
+  _ : inv_submitted_broadcast psent st;
+  _ : inv_conf_lightconfmsg psent st;
+  _ : inv_conf_confmsg psent st;
+  _ : inv_nsigs_correct psent st; (* requires inv_buffer_received *)
+  _ : inv_rlcerts_correct psent st;
+  _ : inv_rcerts_correct psent st;
+  _ : inv_buffer_received psent st;
+}.
+
+(*
+Fact l2h_invariants_pre : is_invariant_reachable_step
+  (fun w => forall n, is_byz n = false -> 
+    inv_buffer_received (sentMsgs w) (w @ n) /\ inv_nsigs_correct (sentMsgs w) (w @ n)).
+Proof.
+  hnf; intros qq ?? Hw H Hstep. pose proof (ReachableStep Hstep Hw) as Hw'.
+  unfold lift_node_inv in *.
+  intros n Hnonbyz. saturate_assumptions!. destruct H as (H & H0).
+  (* TODO this is cumbersome! *)
+  pose proof (id_coh_is_invariant Hw n) as Hcoh.
+  pose proof (id_coh_is_invariant Hw' n) as Hcoh'.
+  pick inv_submit_mixin as_ Hmx' by_ (pose proof (state_invariants Hw n) as []). rewrite Hcoh in Hmx'.
+  assert ((w @ n).(submitted_value) = None -> (w @ n).(from_set) = nil) as Hmx by (now destruct ((w @ n).(submitted_value))). clear Hmx'.
+  pick buffer_nil_after_submit as_ Hbn by_ (pose proof (state_invariants Hw n) as []).
+  (* get the effect *)
+  pose proof Hstep as Hstep_.
+  apply state_mnt_sound with (n:=n) in Hstep.
+  destruct Hstep as (l & Hpsent & _).
+  (* generalize a little bit *)
+  (* TODO put this before? *)
+  assert (exists others, incl others (buffer_augment n (msg_buffer (w @ n))) /\ 
+    psent_effect_star n (sentMsgs w') others l) as Hpsent'.
+  { eexists. split; [ | apply Hpsent ]. destruct qq; hnf; simpl; tauto. }
+  clear Hpsent. destruct Hpsent' as (others & Hincl & Hpsent).
+  hnf in H, H0.
+  split_and?.
+  all: hnf; rewrite Hcoh in *; rewrite Hcoh' in *.
+  1: intros (n0, msg0) Hin; specialize (H (n0, msg0)); clear H0 Hbn Hmx.
+  (* TODO why if we do not specialize here, things will not go through? *)
+  (* TODO revert others? *)
+  2: intros v Hv n0 lsig sig; pose proof (fun vv Hvv => H0 vv Hvv n0 lsig sig) as H'; specialize (H (n0, SubmitMsg v lsig sig));
+    clear H0; rename H' into H0; revert others Hincl Hpsent.
+  (* all: remember (w @ n) as st eqn:Est; remember (w' @ n) as st' eqn:Est'. *)
+  all: (* revert Est' Est; *) induction l as [ st | st d st' l IH ]; intros; saturate_assumptions!.
+  all: (* all MNTnil (under-specified) cases *)
+    try solve [ eapply system_step_psent_norevert_full; eauto ].
+  all: simpl in Hpsent; destruct Hpsent as (Hpsent & HH).
+  all: destruct d; simpl in Hpsent, IH, (type of l); saturate_assumptions; simplify_eq.
+  all: unfold zip_from_lsigs, zip_from_lsigs_sigs, zip_from_sigs in *; simpl in *.
+  all: try solve [ tauto | apply IH; auto with datatypes | apply IH with (others:=others); auto with datatypes ].
+  (* try unify submitted value *)
+  all: pose proof (persistent_invariants_pre l) as ([] & _); 
+    pick submitted_value_persistent as_ Hvv; pick conf_persistent as_ Hcc; simpl in Hvv, Hcc;
+    try (saturate_assumptions! in_ Hvv); try (saturate_assumptions! in_ Hcc).
+  all: try (specialize (Hvv _ eq_refl); rewrite Hvv in * ); simplify_eq.
+  - (* use persistence here *)
+    pick msg_buffer_nil_persistent as_ Hb by_ (pose proof (persistent_invariants_pre l) as ([] & _)). 
+    simpl in Hb. saturate_assumptions. rewrite Hb in Hin. contradiction.
+  - destruct (ListFacts.prod_eq_dec Address_eqdec Message_eqdec (n0, msg0) (src0, SubmitMsg v lsig sig)); simplify_eq; auto.
+    apply IH; auto with datatypes. intros [ | ]; auto; congruence.
+  - apply IH with (others:=nil); try contradiction; auto with datatypes.
+    + (* by contradiction *)
+      rewrite Hmx. simpl. intros. contradiction.
+    + admit.
+  - match goal with Hpsent : In (mkP ?srca _ (SubmitMsg _ ?lsiga ?siga) _) _ \/ In _ _ 
+      |- In (mkP ?srcb _ (SubmitMsg _ ?lsigb ?sigb) _) _ => 
+      destruct (ListFacts.prod_eq_dec (ListFacts.prod_eq_dec Address_eqdec LightSignature_eqdec) Signature_eqdec 
+        (srca, lsiga, siga) (srcb, lsigb, sigb)); try simplify_eq end.
+    + (* prove that others = nil *)
+      destruct Hpsent as [ Hpsent | Hpsent ]; auto.
+      isSome_rewrite. saturate_assumptions. rewrite Hbn in Hincl. simpl in Hincl. now apply Hincl in Hpsent.
+    + eapply IH; eauto; try congruence. intros ? HH1. intros. rewrite HH1 in *. simplify_eq. 
+      eapply H0; try reflexivity. tauto.
+  - destruct (ListFacts.prod_eq_dec Address_eqdec Message_eqdec (n0, SubmitMsg v lsig sig) (src0, SubmitMsg v0 lsig0 sig0)); simplify_eq; auto.
+    eapply IH with (others:=others); eauto with datatypes. 2: now isSome_rewrite. 
+    intros [ | ]; auto; congruence.
+Admitted.
+*)
+Fact l2h_invariants_pre : is_invariant_reachable_step_under
+  (fun w => id_coh w /\ lift_state_inv node_state_invariants w /\ lift_node_inv inv_buffer_received w)
+  (lift_node_inv node_psent_l2h_invariants).
+Proof.
+  hnf; intros qq ?? Hw _ (Hcoh & Hst & Hrcv) (Hcoh' & _ & _) H Hstep.
+  intros n Hnonbyz. (* saturate later *)
+  pose proof (Hcoh n) as Hcoh_. pose proof (Hcoh' n) as Hcoh_'. (* required for bridging n and id later *)
+  (* get the effect *)
+  pose proof Hstep as Hstep_.
+  apply state_mnt_sound with (n:=n) in Hstep; auto.
+  destruct Hstep as (l & Hpsent & _).
+  constructor; auto.
+  7: eapply inv_buffer_received_only; eauto. 7: intros n0; split_and?; auto. 7: destruct (Hst n0); hypothesis. (* requires Hw here *)
+  all: unfold lift_node_inv in *; saturate_assumptions! in_ Hrcv; saturate_assumptions! in_ H.
+  all: match goal with |- ?def _ _ => pick def as_ H' by_ (destruct H); clear H; rename H' into H end.
+  all: hnf; rewrite Hcoh_ in *; rewrite Hcoh_' in *.
+  (* TODO why if we do not specialize here, things will not go through? *)
+  1-4: intros v; specialize (H v).
+  2,3: pick confirmed_then_submitted as_ Hcs by_ (pose proof (Hst n) as []). (* eliminate the Msubmit case *)
+  4: intros Hv n0 lsig sig; revert Hv; pose proof (fun Hy => H Hy n0 lsig sig) as H'; clear H; rename H' into H.
+  4: pick inv_submit_mixin as_ Hmx by_ (pose proof (Hst n) as []); apply inv_submit_mixin_break in Hmx; unfold inv_submit_none in Hmx.
+  4: hnf in Hrcv; rewrite Hcoh in Hrcv; specialize (Hrcv (n0, SubmitMsg v lsig sig)).
+  5: intros lc; specialize (H lc).
+  6: intros c; specialize (H c).
+  all: match goal with |- context[zip_from_lsigs_sigs] => idtac | _ => clear Hrcv end. (* Hrcv will only be used in one goal *)
+  all: intros.
+  all: induction l as [ st | st d st' l IH ]; saturate_assumptions!.
+  all: (* all MNTnil (under-specified) cases *)
+    try solve 
+    [ eapply system_step_psent_norevert_full; eauto
+    | destruct H as (tmp & H); exists tmp; eapply system_step_psent_norevert_full; eauto
+    | eapply system_step_psent_persistent_weak_full; eauto ].
+  all: simpl in Hpsent; destruct Hpsent as (Hpsent & HH).
+  all: destruct d; simpl in Hpsent, IH, (type of l); saturate_assumptions; simplify_eq.
+  all: match type of Hpsent with _ /\ _ => destruct Hpsent as (Hpsent & Hbb) | _ => idtac end. (* for two kinds of special psent_effects *)
+  all: try solve [ tauto | apply IH; auto with datatypes ].
+  (* try unify submitted value *)
+  all: pose proof (persistent_invariants_pre l) as ([] & _); 
+    pick submitted_value_persistent as_ Hvv; pick conf_persistent as_ Hcc; simpl in Hvv, Hcc;
+    try (saturate_assumptions! in_ Hvv); try (saturate_assumptions! in_ Hcc).
+  all: try (specialize (Hvv _ eq_refl); rewrite Hvv in * ); simplify_eq.
+  all: try solve
+    [ match goal with HH : context[?a = ?b \/ In _ _] |- _ => (* new Ins *)
+      first [ destruct (LightCertificate_eqdec a b) as [ <- | ]
+            | destruct (Certificate_eqdec a b) as [ <- | ] ]; try tauto; try eauto end
+    | exists false; apply Hpsent, In_broadcast; eauto (* bcast *)
+    | try isSome_rewrite; try is_true_rewrite; apply IH; auto; eqsolve (* when just use IH *) ].
+  all: unfold zip_from_lsigs, zip_from_lsigs_sigs, zip_from_sigs in *.
+  - (* use persistence *)
+    pick conf_collected_lightsigs_persistent as_ Hll.
+    simpl in Hll. saturate_assumptions. rewrite <- Hll in *. 
+    exists false; apply Hpsent, In_broadcast; eauto.
+  (* FIXME: read the following two cases *)
+  - isSome_rewrite. match_option_rewrite.
+    destruct (lightcert_conflict_check _) in Hbb, IH; saturate_assumptions.
+    + (* use persistence *)
+      pick conf_collected_sigs_persistent as_ Hll1. pick conf_from_set_persistent as_ Hll2.
+      simpl in Hll1, Hll2. saturate_assumptions. unfold zip_from_sigs. rewrite <- Hll1, <- Hll2. 
+      exists false; apply Hbb, In_broadcast; eauto.
+    + apply IH; auto; eqsolve.
+  - destruct (conf st) eqn:?; saturate_assumptions. 2: apply IH; auto; eqsolve.
+    destruct (lightcert_conflict_check _) in Hbb, IH; saturate_assumptions. 2: apply IH; auto; eqsolve.
+    destruct (submitted_value st) as [ v' | ] eqn:?; try discriminate; saturate_assumptions!.
+    rewrite Hvv in *. simplify_eq.
+    (* TODO repeating *)
+    (* use persistence *)
+    pick conf_collected_sigs_persistent as_ Hll1. pick conf_from_set_persistent as_ Hll2.
+    simpl in Hll1, Hll2. saturate_assumptions. unfold zip_from_sigs. rewrite <- Hll1, <- Hll2. 
+    exists false; apply Hbb, In_broadcast; eauto.
+  - (* use IH and show that from = nil *)
+    unfold inv_buffer_received in IH. simpl in IH. apply IH; auto; try contradiction.
+    rewrite Hmx. simpl. contradiction.
+  - (* compare & check if can use IH *)
+    destruct (ListFacts.prod_eq_dec Address_eqdec Message_eqdec (n0, SubmitMsg v lsig sig) (src0, SubmitMsg v lsig0 sig0)); simplify_eq; auto.
+    eapply IH; eauto with datatypes. 2: congruence.
+    intros _ [ | ]; auto; congruence.
+  - (* compare & check if can use IH *)
+    destruct (ListFacts.prod_eq_dec Address_eqdec Message_eqdec (n0, SubmitMsg v lsig sig) (src0, SubmitMsg v0 lsig0 sig0)); simplify_eq; auto.
+    apply IH; auto with datatypes. intros [ | ]; auto; congruence.
+Qed.
+
+Fact l2h_invariants : always_holds (lift_node_inv node_psent_l2h_invariants).
+Proof.
+  eapply is_invariant_reachable_step_under_closed.
+  1: apply l2h_invariants_pre.
+  2: rewrite ! always_holds_and; auto using id_coh_always_holds, state_invariants, inv_buffer_received_always_holds.
+  hnf. intros. constructor; hnf; try discriminate; try contradiction.
+Qed.
+
+End Forward.
+
+Section Backward.
+
+(* the state-major view is useful, but we also need a packetsoup-major view *)
+
+Inductive psent_mnt_type_base (psent : PacketSoup) : Type :=
+  | Pid : psent_mnt_type_base psent
+  | Puse : forall p, In p psent -> psent_mnt_type_base psent
+.
+
+(* ... this design of mixing user packets and Byzantine packets is not good *)
+(*
+Inductive packets_shape_user : Type := PSUbcast (n : Address) (m : Message).
+
+Inductive packets_shape : Type := PSHuser (psu : packets_shape_user) | PSHbyz (p : Packet).
+*)
+
+(* intended to be in a module type, or something, provided by user *)
+Inductive packets_shape : Type := PSbcast (n : Address) (m : Message).
+
+Definition packets_shape_consistent (ps : packets_shape) (pkts : list Packet) : Prop :=
+  match ps with
+  | PSbcast n m => pkts = broadcast n m
+  end.
+
+(* a list *)
+(* the base psent will not change, which represents the psent before update *)
+(* ... this design is not very good, since the cons part can be just a normal list *)
+(*
+Inductive psent_mnt_type : PacketSoup -> Type :=
+  | Pbase : forall psent, psent_mnt_type_base psent -> psent_mnt_type psent
+  | Pcons : forall pkts ps,
+    Forall (fun p => p.(consumed) = false) pkts ->
+    packets_shape_consistent ps pkts ->
+    forall psent, psent_mnt_type psent -> psent_mnt_type psent
+  (* HMM since we are proving, do not consider sendout1 ...? *)
+.
+
+Global Arguments Pbase : clear implicits.
+Global Arguments Pcons : clear implicits.
+*)
+
+(* want to write it in another way so that the base part can be exposed, 
+    which will enable some proofs about psent_mnt_type concatenation *)
+(* write the atomic part as a dependent record? *)
+(* FIXME: this is a strong over-approximation; actually, the sender (which is unique
+    in one transition) should be the argument. but now we do not need that precise
+    description so skip *)
+Record psent_mnt_type : Type := mkPMT {
+  pkts : list Packet;
+  ps : packets_shape;
+  _ : Forall (fun p => p.(consumed) = false) pkts;
+  _ : packets_shape_consistent ps pkts;
+}.
+
+Global Arguments mkPMT : clear implicits.
+
+Definition psent_mnt_base psent (s : psent_mnt_type_base psent) : PacketSoup :=
+  match s with
+  | Pid _ => psent
+  | Puse _ p _ => consume p psent
+  end.
+
+(* intuitively, psent' gets smaller when l gets smaller *)
+Fixpoint psent_mnt psent (b : psent_mnt_type_base psent) (l : list psent_mnt_type) psent' : Prop :=
+  match l with
+  | nil => 
+    (* psent' = psent_mnt_base b *)
+    Ineq psent' (psent_mnt_base b)
+  | a :: l' => exists psent_, psent_mnt b l' psent_ /\ Ineq psent' (sendout a.(pkts) psent_)
+  end.
+
+Fact psent_mnt_idbase_Ineq [psent psent1 psent2] (l : list psent_mnt_type) (H : Ineq psent1 psent2) :
+  psent_mnt (Pid psent1) l psent <-> psent_mnt (Pid psent2) l psent.
+Proof.
+  revert psent. induction l; simpl; intros.
+  - now rewrite H.
+  - setoid_rewrite IHl. auto.
+Qed.
+
+Fact psent_mnt_result_Ineq [psent psent1 psent2] (b : psent_mnt_type_base psent) (l : list psent_mnt_type) (H : Ineq psent1 psent2) :
+  psent_mnt b l psent1 <-> psent_mnt b l psent2.
+Proof.
+  destruct l as [ | a l' ]; simpl.
+  - now rewrite H.
+  - setoid_rewrite H. auto.
+Qed.
+
+Fact psent_mnt_base_change [psent psent'] (b : psent_mnt_type_base psent) (l : list psent_mnt_type) :
+  psent_mnt b l psent' <-> psent_mnt (Pid (psent_mnt_base b)) l psent'.
+Proof.
+  revert psent'. induction l as [ | a l IH ]; simpl; intros.
+  - reflexivity.
+  - setoid_rewrite IH. reflexivity.
+Qed.
+
+Fact psent_mnt_idbase_pop [psent psent'] l a :
+  psent_mnt (Pid (sendout a.(pkts) psent)) l psent' <-> psent_mnt (Pid psent) (l ++ a :: nil) psent'.
+Proof.
+  revert psent'. induction l as [ | a' l IH ]; simpl; intros.
+  - split. 
+    + intros HH. exists psent. split; try reflexivity; auto.
+    + intros (psent_ & Ha & Hb). hnf in Ha, Hb |- *. intros x. specialize (Ha x). specialize (Hb x).
+      autorewrite with psent in Ha, Hb |- *. tauto.
+  - setoid_rewrite IH. auto.
+Qed.
+
+(* here, the list to be appended must start with Pid *)
+Fact psent_mnt_append [psent psent' psent''] (b : psent_mnt_type_base psent) (l l' : list psent_mnt_type)
+  (H : psent_mnt b l psent') (H' : psent_mnt (Pid psent') l' psent'') : psent_mnt b (l' ++ l) psent''.
+Proof.
+  revert l psent b psent' psent'' H H'. induction l' as [ | a l' IH ]; simpl; intros.
+  - erewrite psent_mnt_result_Ineq by eassumption. assumption.
+  - destruct H' as (psent_ & H1 & H2). saturate_assumptions!. eauto.
+Qed.
+
+(* TODO the following functions seems to be repeating the bodies of the h2l invariants above. 
+  maybe put these above and reuse? *)
+Definition state_effect_bcast (n : Address) (m : Message) (stmap : StateMap) : Prop :=
+  let: st := (stmap n) in
+  match m with
+  | SubmitMsg v lsig sig => 
+    verify v sig n /\ light_verify v lsig n /\
+    st.(submitted_value) = Some v
+  | LightConfirmMsg (v, cs) =>
+    st.(conf) /\ st.(submitted_value) = Some v /\
+    cs = lightsig_combine st.(collected_lightsigs)
+  | ConfirmMsg (v, nsigs) => 
+    st.(conf) /\ lightcert_conflict_check st.(received_lightcerts) (* this is new *)
+    /\ st.(submitted_value) = Some v /\ nsigs = zip_from_sigs st
+  end.
+
+Definition state_effect_recv (src : Address) (m : Message) (st : State) : Prop :=
+  (* currently only uses single point, so reduces the argument *)
+  (* let: st := (stmap n) in *)
+  match m with
+  | SubmitMsg v lsig sig => 
+    match st.(submitted_value) with
+    | None => In (src, m) st.(msg_buffer)
+    | Some ov => 
+      (* the length condition may be more natural, but it would be hard to reason about 
+        without invariant 1; so replace it with the condition on conf *)
+      (* length st.(from_set) < N - t0 -> *)
+      st.(conf) = false ->
+      v = ov -> verify v sig src -> light_verify v lsig src ->
+        In src st.(from_set) (* ths should be enough *)
+    end
+  | LightConfirmMsg (v, cs) =>
+    combined_verify v cs -> In (v, cs) st.(received_lightcerts)
+  | ConfirmMsg (v, nsigs) => 
+    certificate_valid v nsigs -> NoDup nsigs -> (N - t0 <= (length nsigs)) ->
+    In (v, nsigs) st.(received_certs)
+  end.
+
+(* here, stmap refers to the updated state map *)
+(* it seems not quite useful to constrain on the original state map *)
+(* writing this as an inductive prop will make inversion difficult;
+    for example, inverting "state_effect stmap (Pcons pkts H psent l)" will not give "state_effect stmap l", 
+    due to some weird reason ...
+  use another way to constrain the shape of pkts, instead *)
+
+(* TODO if this works, consider how to distribute the constraints here and in "psent_mnt_type"
+    of course, constraints involving stmap must be here *)
+Definition state_effect_base [psent] (stmap : StateMap) (b : psent_mnt_type_base psent) : Prop :=
+  match b with
+  | Pid _ => True (* under-specified *)
+  | Puse _ (mkP src n m used) _ => is_byz n = false /\ state_effect_recv src m (stmap n)
+  end.
+
+Global Arguments state_effect_base [_] _ !_.
+
+Fixpoint state_effect_send (stmap : StateMap) (l : list psent_mnt_type) : Prop :=
+  match l with
+  | nil => True
+  | a :: l' =>
+    state_effect_send stmap l' /\ (* putting this here can be convenient *)
+    match a.(ps) with
+    | PSbcast n m => is_byz n = false /\ state_effect_bcast n m stmap
+    end
+  end.
+
+Fact state_effect_send_app stmap l l' : 
+  state_effect_send stmap (l ++ l') <-> state_effect_send stmap l /\ state_effect_send stmap l'.
+Proof. revert l'. induction l; simpl; intros; try tauto. rewrite IHl. tauto. Qed.
+
+Fact state_effect_bcast_stmap_peq stmap stmap' n msg (Hpeq : forall n, stmap n = stmap' n) : 
+  state_effect_bcast n msg stmap <-> state_effect_bcast n msg stmap'.
+Proof. destruct msg; simpl. all: rewrite Hpeq; auto. Qed.
+
+Fact state_effect_send_stmap_peq stmap stmap' l (Hpeq : forall n, stmap n = stmap' n) : 
+  state_effect_send stmap l <-> state_effect_send stmap' l.
+Proof. induction l; simpl; intros; try tauto. rewrite IHl. destruct (ps _). rewrite state_effect_bcast_stmap_peq by eassumption. tauto. Qed.
+
+Inductive psent_sender_kind (psent : list Packet) : Type := 
+  | PSKnonbyz (b : psent_mnt_type_base psent) (l : list psent_mnt_type)
+  | PSKbyz (p : Packet).
+
+Definition state_effect (stmap : StateMap) [psent] (psk : psent_sender_kind psent) : Prop :=
+  match psk with
+  | PSKnonbyz b l => state_effect_base stmap b /\ state_effect_send stmap l
+  | PSKbyz _ p => is_byz p.(src) /\ p.(consumed) = false /\ byz_constraints p.(msg) (mkW stmap psent) (* FIXME: is byz_constraints only about psent? *)
+  end.
+
+Ltac state_effect_solve :=
+  simpl; eauto; repeat (first [ rewrite upd_refl; simpl ]); split_and?; 
+  try isSome_rewrite; try tauto; try eqsolve; auto.
+
+(* here, do not consider base *)
+(* FIXME: unify with the one in RB? *)
+Ltac psent_analyze' psent' :=
+  match psent' with
+  | sendout (?pkts1 ++ ?pkts2) ?psent_ =>
+    let ss := psent_analyze' constr:(sendout pkts1 psent_) in
+    match pkts2 with
+    | broadcast ?n ?m => uconstr:((mkPMT pkts2 (PSbcast n m) (broadcast_all_fresh n m) eq_refl) :: ss)
+    end
+  | sendout ?pkts ?psent_ => 
+    let ss := psent_analyze' constr:(psent_) in
+    match pkts with
+    | broadcast ?n ?m => uconstr:((mkPMT pkts (PSbcast n m) (broadcast_all_fresh n m) eq_refl) :: ss)
+    end
+  (*
+  | sendout1 ?p ?psent_ => 
+    (* early terminate *)
+    uconstr:((mkPMT (p :: nil) (PSHbyz p) ltac:(now constructor) eq_refl) :: nil)
+  *)
+  | _ => uconstr:(@nil psent_mnt_type)
+  end.
+
+Ltac psent_mnt_solve :=
+  match goal with
+  (*
+  | |- exists (_ : _), _ = _ /\ _ => 
+    eexists; split; (* TODO appending anything after the semicolon here will result in non-termination? *)
+    *)
+  | |- exists (_ : _), (* _ = ?psent *) (Ineq _ ?psent) /\ _ => exists psent; split; 
+    (* [ reflexivity | solve [ reflexivity (*| intros ?; autorewrite with psent; tauto ]*) ] ] *)
+    (* does not work ... *)
+    [ reflexivity | ];
+    first [ reflexivity | intros ?; autorewrite with psent; simpl; tauto | idtac ]
+    (* why the last tactic may not work? *)
+  | |- exists (_ : _), (exists _, _) /\ _ => 
+    eexists; split; [ psent_mnt_solve | intros ?; autorewrite with psent ]; try tauto
+  | _ => idtac
+  end.
+
+Ltac psent_analyze :=
+  try rewrite sendout0;
+  match goal with
+  | |- exists (_ : ?t), psent_mnt _ _ ?psent' /\ _ =>
+    let l := psent_analyze' psent' in
+    unshelve eexists l;
+    match goal with
+    | |- psent_mnt _ _ ?psent' /\ _ => 
+      split; [ simpl; auto; try reflexivity; psent_mnt_solve | state_effect_solve ]
+    (* | _ => try apply broadcast_all_fresh *)
+    | _ => idtac
+    end
+  end.
+
+Definition lift_pkt_inv' (P : Packet -> StateMap -> Prop) : PacketSoup -> StateMap -> Prop :=
+  fun psent stmap => forall p, In p psent -> P p stmap.
+
+Definition lift_pkt_inv (P : Packet -> StateMap -> Prop) : World -> Prop :=
+  Eval unfold lift_pkt_inv' in fun w => lift_pkt_inv' P (sentMsgs w) (localState w).
+
+Fact psent_mnt_sound_pre_pre p (Hnonbyz : is_byz (dst p) = false) stf msf w w'
+  (Hcoh : id_coh w) (* still needed *)
+  (Ef : procMsgWithCheck (w @ dst p) (src p) (msg p) = (stf, msf))
+  psent (E0 : w' = mkW (upd (dst p) stf (localState w)) (sendout msf psent)) (Hpin : In p psent) :
+  exists l : list psent_mnt_type,
+    psent_mnt (Pid psent) l (sentMsgs w') /\ state_effect (localState w') (PSKnonbyz (Puse psent p Hpin) l).
+    (* /\ (lift_pkt_inv' inv_submitmsg_receive psent (localState w) ->
+      lift_pkt_inv' inv_submitmsg_receive (sendout msf psent) (localState w')). *)
+Proof.
+  destruct p as [ src dst msg used ]. simpl_pkt. subst w'. simpl. unfold procMsgWithCheck in Ef. 
+  destruct_localState w dst as_ [ ? conf ov from lsigs sigs rlcerts rcerts buffer ] eqn_ Est.
+  destruct msg as [ v ls s | (v, cs) | (v, nsigs) ]; simpl in Ef; simplify_eq. (* pair inj *)
+  + destruct ov as [ vthis | ].
+    (* TODO a tactic for sumbool rewriting *)
+    * destruct (andb _ _) eqn:EE in Ef; unfold is_left in EE; 
+        [ rewrite !andb_true_iff, sumbool_is_left in EE
+        | rewrite !andb_false_iff, sumbool_is_right in EE ]; simplify_eq.
+      2: psent_analyze.
+      destruct EE as ((-> & Everi) & Elveri).
+      destruct conf eqn:?.
+      --simplify_eq. simpl. 
+        destruct (lightcert_conflict_check _) eqn:? in |- *; simpl.
+        all: psent_analyze. 
+      --destruct (in_dec _ _ _) as [ Hin | Hnotin ] in Ef; simplify_eq.
+        1: psent_analyze. 
+        simpl.
+        destruct (N - t0 <=? S (length from)) eqn:Eth; simpl;
+          [ apply Nat.leb_le in Eth | apply Nat.leb_nle in Eth ].
+        1: destruct (lightcert_conflict_check _) eqn:? in |- *; simpl.
+        all: psent_analyze.
+    * simplify_eq. simpl. psent_analyze.
+  + destruct (combined_verify _ _) eqn:EE in Ef; simplify_eq.
+    2: psent_analyze.
+    simpl. rewrite app_nil_r. 
+    destruct ov in |- *; [ destruct (andb _ _) eqn:EE0 in |- *; 
+      [ rewrite andb_true_iff in EE0 | rewrite andb_false_iff in EE0 ]; destruct EE0; try is_true_rewrite | ]; simpl.
+    all: psent_analyze.
+  + destruct (andb _ _) eqn:EE in Ef; unfold is_left in EE; 
+      [ rewrite !andb_true_iff, !sumbool_is_left, !Nat.leb_le in EE
+      | rewrite !andb_false_iff, !sumbool_is_right, !Nat.leb_nle in EE ]; simplify_eq.
+    all: psent_analyze.
+Qed.
+(*
+Fact psent_mnt_sound_pre q w w' (Hstep : system_step q w w') (Hq_ : forall n t, q <> Intern n t) 
+  (* having reachable instead would complicate the induction proof *)
+  (Hcoh : id_coh w) (* still needed *) :
+  exists (b : psent_mnt_type_base (sentMsgs w)) (l : list psent_mnt_type),
+    psent_mnt b l (sentMsgs w') /\ state_effect (localState w') b l.
+Proof.
+  inversion_step' Hstep; clear Hstep; intros.
+  3: exfalso; eapply Hq_; reflexivity.
+  - exists (Pid _). psent_analyze.
+  - exists (Puse _ _ Hpin).
+    let pkt := constr:(mkP src dst msg used) in
+      eapply psent_mnt_sound_pre_pre with (psent:=consume pkt (sentMsgs w)) in Ef; try reflexivity; auto.
+    simpl in Ef. destruct Ef as (l & Ha & Hb).
+    exists l. rewrite psent_mnt_base_change. simpl. 
+    exists ( 
+  - (* TODO the bug happens here ... *)
+    psent_analyze. (* ???? *)
+    intros ?; autorewrite with psent; simpl; tauto.
+Qed.
+*)
+(* required below? *)
+
+Fact procMsgWithCheck_fresh st src m :
+  Forall (fun p => p.(consumed) = false) (snd (procMsgWithCheck st src m)).
+Proof with (simpl; rewrite ?Forall_app; auto using broadcast_all_fresh).
+  unfold procMsgWithCheck, routine_check.
+  destruct st as [ n conf ov from lsigs sigs rlcerts rcerts buffer ], m as [ v lsig sig | (v, cs) | (v, nsigs) ]; simpl.
+  - destruct ov...
+    destruct (andb _ _)... destruct conf.
+    + destruct (andb _ _)...
+    + destruct (in_dec _ _ _)...
+      destruct (andb _ _). all: destruct (Nat.leb _ _)...
+  - destruct (combined_verify _ _)...
+    destruct ov... destruct (andb _ _)...
+  - destruct (andb _ _)...
+Qed.
+
+(* specialized to this invariant only *)
+(*
+Fact inv_submitmsg_receive_fresh_skip psent psent' pkts st
+  (Hf : Forall (fun p => p.(consumed) = false) pkts) (Hpsent : forall p, In p psent' <-> In p psent \/ In p pkts) :
+  (forall p, In p psent -> inv_submitmsg_receive_ p st) ->
+  (forall p, In p psent' -> inv_submitmsg_receive_ p st).
+Proof.
+  intros H p Hin%Hpsent. destruct Hin as [ Hin | Hin ]; auto.
+  eapply Forall_forall in Hin. 2: apply Hf. simpl in Hin. hnf. rewrite Hin. now destruct (msg p).
+Qed.
+*)
+Fact psent_mnt_sound_pre n t w w' (Hstep : system_step (Intern n t) w w') (Hw : reachable w) :
+  (lift_pkt_inv' inv_submitmsg_receive (sentMsgs w) (localState w) ->
+    lift_pkt_inv' inv_submitmsg_receive (sentMsgs w') (localState w')) /\
+  exists l : list psent_mnt_type,
+    psent_mnt (Pid (sentMsgs w)) l (sentMsgs w') /\ state_effect (localState w') (PSKnonbyz (Pid (sentMsgs w)) l).
+Proof.
+  simpl.
+  pose proof (id_coh_always_holds Hw) as Hcoh.
+  (* destruct q as [ | | n t | ]. 
+  1,2,4: eapply psent_mnt_sound_pre; try eassumption; auto. *)
+  inversion_step' Hstep; clear Hstep; intros; try discriminate.
+  revert Hq. intros [= <-]. destruct t1.
+  pose proof (inv_buffer_received_always_holds Hw Hnonbyz) as Hrcv. hnf in Hrcv. 
+  destruct_localState w n as_ [ ? conf ov from lsigs sigs rlcerts rcerts buffer ] eqn_ Est. simpl_state.
+  simpl in E.
+  (* destruct ov. 1: simplify_eq; psent_analyze. *)
+  destruct ov. 1: simplify_eq; split; [ | psent_analyze ].
+  1:{ rewrite sendout0. intros Hq. hnf in Hq |- *. intros p Hin. specialize (Hq _ Hin). 
+    unfold inv_submitmsg_receive in Hq |- *. now rewrite <- Est, -> upd_intact. }
+  destruct (fold_right _ _ _) as (st_, ps_) eqn:Efr in E. simplify_eq.
+  change (set _ _ (set _ _ _)) with (Node n conf (Some (value_bft n)) from lsigs sigs rlcerts rcerts nil) in Efr.
+  (* time to do induction *)
+  assert (st'.(id) = n /\ (* required by psent_mnt_sound_pre_pre *)
+    st'.(submitted_value) = Some (value_bft n) /\ (* required at the end *)
+    Forall (fun '(src, msg) => state_effect_recv src msg st') buffer /\
+    Forall (fun p => p.(consumed) = false) ps_ /\ (* required to do fresh skip *)
+    exists l : list psent_mnt_type, 
+    psent_mnt (Pid (sentMsgs w)) l (sendout ps_ (sentMsgs w)) /\ state_effect_send (upd n st' (localState w)) l) as Hgoal.
+  { clear Est. revert st' ps_ Efr. induction buffer as [ | (src, msg) buffer IH ]; intros; simpl in Efr.
+    - simplify_eq. split_and?; auto. psent_analyze.
+    - destruct (procMsgWithCheck _ _ _) as (sta, psa) eqn:E0 in Efr.
+      destruct (fold_right _ _ _) as (stb, psb) eqn:E1 in Efr. rewrite E1 in E0. simpl in E0, Efr. 
+      revert Efr. intros [= <- <-].
+      simpl in Hrcv. specialize (IH (fun a H => Hrcv a (or_intror H))).
+      saturate_assumptions! in_ IH. destruct IH as (Hcohb & Hvb & Hre & Hfresh & l & Ha & HH).
+      (* use the previous lemma to obtain persistence ... TODO this is cumbersome, any better way? *)
+      specialize (Hrcv _ (or_introl eq_refl)). simpl in Hrcv.
+      epose proof (DeliverStep (Deliver (mkP src n msg true)) (mkW (upd n stb (localState w)) (sentMsgs w))
+        _ _ eq_refl Hrcv Hnonbyz ?[Goalq]) as H.
+      [Goalq]: simpl; rewrite upd_refl, E0; reflexivity.
+      eapply state_mnt_sound_pre_pre with (n:=n) in H; auto. simpl in H. destruct H as (ll & _). rewrite !upd_refl in ll.
+      pose proof (persistent_invariants_pre ll) as ([] & _).
+      split; try congruence.
+      apply and_wlog_r. 1: hnf in *; auto. intros Hva.
+      (* use previous lemma *)
+      epose proof (@psent_mnt_sound_pre_pre (mkP src n msg true) Hnonbyz sta psa
+        (mkW (upd n stb (localState w)) nil (* not important *)) _ ?[Goalq] ltac:(simpl; rewrite upd_refl; assumption)
+        (sendout psb (sentMsgs w)) eq_refl ltac:(rewrite In_sendout; now right)) as Hgoal.
+      [Goalq]:{ hnf. simpl. intros n0. unfold upd. destruct (Address_eqdec _ _); auto; congruence. }
+      simpl in Hgoal. destruct Hgoal as (l0 & Ha0 & ((_ & Hre0) & HH0)). rewrite !upd_refl in Hre0.
+      (* well, this is inevitable *)
+      split.
+      1:{ constructor; auto. revert Hre. apply Forall_impl. intros (src0, [ v0 lsig0 sig0 | (v0, cs0) | (v0, nsigs0) ]) Htmp.
+        all: simpl in Htmp |- *; intros; try (rewrite Hvb in Htmp; rewrite Hva); intros.
+        all: hnf in *; try is_true_rewrite; intuition.
+        destruct (ACP.conf stb); saturate_assumptions; try discriminate. intuition. }
+      split.
+      1:{ apply Forall_app. split; auto. epose proof (procMsgWithCheck_fresh _ _ _) as Htmp. now rewrite E0 in Htmp. }
+      (* compose *)
+      pose proof (psent_mnt_append _ _ _ Ha Ha0) as Hq.
+      exists (l0 ++ l). split.
+      + erewrite psent_mnt_result_Ineq. 1: apply Hq.
+        hnf. intros. autorewrite with psent. tauto.
+      + rewrite state_effect_send_app. split.
+        * erewrite state_effect_send_stmap_peq. 1: apply HH0.
+          intros. unfold upd. now destruct_eqdec as_ ?.
+        * (* TODO this is so bad ... *)
+          clear Hq Ha. induction l as [ | a l IH ]; simpl; auto.
+          simpl in HH. destruct HH as (HH & Ht). saturate_assumptions. split; auto.
+          destruct (ps a) as [ n0 [ ? ? ? | (?, ?) | (?, ?) ] ]; simpl in Ht |- *. 
+          all: unfold upd in Ht |- *; destruct_eqdec as_ <-; auto.
+          (* time to use various persistence *)
+          all: hnf in *; unfold zip_from_sigs in *. 
+          all: destruct_and? Ht; split_and?; saturate_assumptions!; auto; try congruence.
+          (* well, ... *)
+          hnf in *. now apply lightcert_conflict_check_persistent with (st:=stb).
+  }
+  destruct Hgoal as (_ & Hv & Hre & Hfresh & l & Ha & HH).
+  (* use the accumulation of state_effect_recv to prove the invariant! *)
+  split.
+  1:{ intros Hq. hnf in Hq |- *. intros p Hin. autorewrite with psent in Hin.
+    unfold inv_submitmsg_receive in Hq |- *. destruct Hin as [ [ Hin | Hin ] | Hin ].
+    - eapply Forall_forall in Hin; try eassumption; simpl in Hin. hnf. rewrite Hin. now destruct (msg p).
+    - apply In_broadcast in Hin; destruct Hin as (? & ->); simpl. apply I.
+    - specialize (Hq _ Hin). unfold upd. destruct p as [ src dst msg used ]. simpl in Hq |- *.
+      destruct (Address_eqdec n dst) as [ <- | ]; auto.
+      rewrite Est in Hq. hnf in Hq |- *. simpl in Hq |- *. rewrite Hv.
+      destruct msg as [ v0 lsig0 sig0 | | ], used; auto.
+      saturate_assumptions. eapply Forall_forall in Hq; try eassumption. simpl in Hq. now rewrite Hv in Hq. }
+  match goal with |- context[SubmitMsg ?v ?lsig ?sig] =>
+    let m := constr:(SubmitMsg v lsig sig) in
+    exists ((mkPMT (broadcast n m) (PSbcast n m) (broadcast_all_fresh n m) eq_refl) :: l) end.
+  split_and?; auto; simpl.
+  - exists (sendout ps_ (sentMsgs w)). split; auto. 
+    hnf. intros ?. autorewrite with psent. tauto.
+  - split_and?; auto with ABCinv.
+    now rewrite upd_refl.
+Qed.
+
+Fact psent_mnt_sound q w w' (Hstep : system_step q w w') (Hw : reachable w) :
+  (lift_pkt_inv' inv_submitmsg_receive (sentMsgs w) (localState w) ->
+    lift_pkt_inv' inv_submitmsg_receive (sentMsgs w') (localState w')) /\
+  exists psk : psent_sender_kind (sentMsgs w),
+    state_effect (localState w') psk /\
+    match psk with
+    | PSKnonbyz b l => psent_mnt b l (sentMsgs w')
+    | PSKbyz _ p => localState w' = localState w (* this should be enough *) /\ sentMsgs w' = sendout1 p (sentMsgs w)
+    end.
+Proof.
+  inversion_step' Hstep.
+  - split; auto. now exists (PSKnonbyz (Pid _) nil).
+  - pose proof (procMsgWithCheck_fresh (w @ dst) src msg) as Hfresh. unfold procMsgWithCheck in Hfresh. rewrite Ef in Hfresh. simpl in Hfresh.
+    pose proof (id_coh_always_holds Hw) as Hcoh.
+    let pkt := constr:(mkP src dst msg used) in
+      unshelve eapply psent_mnt_sound_pre_pre with (p:=receive_pkt pkt) (psent:=consume pkt (sentMsgs w)) in Ef; try reflexivity; auto.
+    1: rewrite In_consume; simpl; tauto.
+    simpl in Ef. destruct Ef as (l & Ha & ((_ & Hre) & Hb)). rewrite upd_refl in Hre.
+    split.
+    (* TODO this proof is kind of repeating *)
+    + intros Hq. hnf in Hq |- *. intros p Hin. autorewrite with psent in Hin.
+      unfold inv_submitmsg_receive in Hq |- *. destruct Hin as [ Hin | Hin ].
+      * eapply Forall_forall in Hin; try eassumption; simpl in Hin. hnf. rewrite Hin. now destruct (P0.msg p).
+      * apply In_consume in Hin. simpl in Hin. destruct Hin as [ <- | (Hin & _) ].
+        --simpl. rewrite upd_refl. hnf. simpl. destruct msg as [ v0 lsig0 sig0 | | ]; auto.
+        --specialize (Hq _ Hin). unfold upd. destruct p as [ src0 dst0 msg0 used0 ]. simpl.
+          destruct (Address_eqdec _ _) as [ <- | ] in |- *; auto.
+          (* here, relies on the fact that receiving does not change the submitted value! *)
+          hnf in Hq |- *. simpl in Hq |- *. destruct msg0 as [ | | ], used0; auto.
+          saturate_assumptions. intros _.
+          eapply state_mnt_sound_pre_pre with (n:=dst) in Hstep; auto.
+          simpl in Hstep. rewrite !upd_refl in Hstep. destruct Hstep as (ll & _ & _ & Hvv). rewrite Hvv in Hq.
+          (* and also some persistence *)
+          pose proof (persistent_invariants_pre ll) as ([] & _). hnf in *.
+          destruct (submitted_value stf); intros; try intuition.
+          destruct (conf (w @ dst)); saturate_assumptions; auto. now is_true_rewrite.
+    + (* this flipping is good *)
+      exists (PSKnonbyz (Puse (sentMsgs w) (mkP src dst msg used) Hpin) l). simpl. rewrite upd_refl.
+      split_and?; try tauto. now rewrite psent_mnt_base_change.
+  - eapply psent_mnt_sound_pre in Hstep; auto.
+    simpl in Hstep. destruct Hstep as (? & l & Hstep). destruct_and? Hstep.
+    split; auto. exists (PSKnonbyz (Pid (sentMsgs w)) l). now simpl.
+  - split.
+    + intros Hq. hnf in Hq |- *. intros p Hin. rewrite In_sendout1 in Hin. 
+      unfold inv_submitmsg_receive in Hq |- *. destruct Hin as [ <- | Hin ]; auto.
+      hnf. simpl. now destruct m.
+    + exists (PSKbyz _ (mkP n dst0 m false)).
+      simpl. now rewrite_w_expand w in_ Hc.
+Qed.
+
+Fact inv_submitmsg_receive_always_holds : always_holds (lift_pkt_inv inv_submitmsg_receive).
+Proof.
+  intros w Hw. induction Hw as [ | q w w' Hstep Hw H ]; auto.
+  - (* TODO streamline the proof here? *)
+    unfold initWorld, initState, Init. hnf. simpl. intros. contradiction.
+  - eapply psent_mnt_sound in H; eauto.
+Qed.
+
+Definition lift_pkt_inv_alt' (P : Packet -> PacketSoup -> Prop) : PacketSoup -> Prop :=
+  fun psent => forall p, In p psent -> P p psent.
+
+Definition lift_pkt_inv_alt (P : Packet -> PacketSoup -> Prop) : World -> Prop :=
+  Eval unfold lift_pkt_inv_alt' in fun w => lift_pkt_inv_alt' P (sentMsgs w).
+
+(* this bunch can pass the base case easily, since it does no work for existing packets *)
+Record node_psent_h2l_invariants_sent_nonbyz p stmap : Prop := {
+  _ : inv_submitmsg_correct p stmap;
+  _ : inv_lightconfirmmsg_correct_nonbyz p stmap;
+  _ : inv_confirmmsg_correct_nonbyz p stmap;
+}.
+
+(* this bunch can pass the base case easily, since it does no work for existing packets *)
+(* sending only, since we do not model the local state of Byz node *)
+Record node_psent_h2l_invariants_byz p history : Prop := {
+  _ : inv_lightconfirmmsg_correct_byz p history;
+  _ : inv_confirmmsg_correct_byz p history;
+}.
+
+(* this is not easy to prove individually, since we need to prove that 
+    all packets sent out in Deliver or Intern transitions are from non-Byz nodes, 
+    which needs another proof *)
+(*
+Fact h2l_invariants_byz :
+  is_invariant_step (lift_pkt_inv_alt node_psent_h2l_invariants_byz).
+Proof with (repeat (progress (hnf in *; intros))); simplify_eq; (repeat (progress (hnf in *; saturate_assumptions!))).
+  hnf. intros ??? H Hstep.
+  hnf in H |- *. intros [ src0 dst0 msg0 used0 ] Hin.
+  inversion_step' Hstep; auto.
+  - constructor; hnf.
+    all: destruct msg0 as [ | (v0, cs0) | (v0, nsigs0) ]; auto; intros...
+*)
+
+(* this bunch can pass the cons case easily, since it does no work for fresh packets *)
+(* for nonbyz only *)
+Record node_psent_h2l_invariants_recv_pre p stmap : Prop := {
+  (* _ : inv_submitmsg_receive p stmap; *)
+  _ : inv_lightconfirmmsg_receive p stmap;
+  _ : inv_confirmmsg_receive p stmap;
+}.
+
+Fact h2l_invariants_id_pre q w w' (Hstep : system_step q w w') (Hw : reachable w) p :
+  (node_psent_h2l_invariants_sent_nonbyz p (localState w) ->
+  forall used, node_psent_h2l_invariants_sent_nonbyz (mkP p.(src) p.(dst) p.(msg) used) (localState w')) /\
+  (node_psent_h2l_invariants_recv_pre p (localState w) ->
+  node_psent_h2l_invariants_recv_pre p (localState w')).
+Proof.
+  destruct p as [ src dst msg used ].
+  pose proof (persistent_invariants Hstep Hw) as Hinv. (* use persistent properties to solve *)
+  split; intros H.
+  1: intros used'; simpl.
+  all: constructor.
+  all: match goal with |- ?def _ _ => pick def as_ H' by_ (destruct H); clear H; rename H' into H;
+    unfold def end.
+  all: destruct msg as [ | (?, ?) | (?, ?) ], used; simpl in *; try exact I.
+  all: pose proof (Hinv src) as []; pose proof (Hinv dst) as [].
+  all: intros; hnf in *; unfold zip_from_sigs in *; saturate_assumptions!; split_and?; destruct_and? H;
+    try isSome_rewrite; try is_true_rewrite; saturate_assumptions; saturate_assumptions!.
+  all: try solve [ eauto using lightcert_conflict_check_persistent | tauto | congruence | intuition ].
+Qed.
+
+Corollary h2l_invariants_id q w w' (Hstep : system_step q w w') (Hw : reachable w) psent :
+  (lift_pkt_inv' node_psent_h2l_invariants_sent_nonbyz psent (localState w) ->
+  lift_pkt_inv' node_psent_h2l_invariants_sent_nonbyz psent (localState w')) /\
+  (lift_pkt_inv' node_psent_h2l_invariants_recv_pre psent (localState w) ->
+  lift_pkt_inv' node_psent_h2l_invariants_recv_pre psent (localState w')).
+Proof.
+  split; intros H; hnf in H |- *; intros [ src dst msg used ] Hin; specialize (H _ Hin).
+  all: now eapply (h2l_invariants_id_pre Hstep Hw) in H; eauto.
+Qed.
+
+Fact h2l_invariants_pre :
+  is_invariant_reachable_step_under id_coh (* needed, since will use psent_mnt_sound *)
+    (fun w => lift_pkt_inv node_psent_h2l_invariants_sent_nonbyz w
+      /\ lift_pkt_inv_alt node_psent_h2l_invariants_byz w
+      /\ lift_pkt_inv node_psent_h2l_invariants_recv_pre w).
+Proof with (repeat (progress (hnf in *; intros))); simplify_eq; (repeat (progress (hnf in *; saturate_assumptions))).
+  hnf; intros q ?? Hw _ Hcoh Hcoh' H Hstep. unfold lift_pkt_inv, lift_pkt_inv_alt in H |- *. 
+  (* get the effect *)
+  pose proof Hstep as Hstep_.
+  apply psent_mnt_sound in Hstep; try assumption.
+  destruct Hstep as (_ & [ b l | [ src dst msg ? ] ] & Hse & Hpsent); simpl in Hse, Hpsent.
+  - (* nonbyz step *)
+    destruct Hse as (Hb & Hse). 
+    remember (sentMsgs w') as psent eqn:Htmp; clear Htmp. (* TODO generalize? *)
+    revert psent Hpsent H Hse. 
+    induction l as [ | a l IH ]; intros.
+    all: simpl in Hse, Hpsent.
+    (* TODO why we do not need to destruct H here (and only need to destruct later)? can I explain? *)
+    + destruct b as [ | p' Hin' ]; simpl in Hb, Hpsent; hnf in Hpsent.
+      * split_and?; intros ?; rewrite Hpsent; revert p; try now apply (h2l_invariants_id Hstep_ Hw (sentMsgs w)).
+        (* byz *)
+        destruct H as (_ & H & _). 
+        intros [ src0 dst0 [ | (v0, cs0) | (v0, nsigs0) ] used0 ] Hin; specialize (H _ Hin); destruct H; hnf in *.
+        all: constructor; hnf; auto...
+        all: setoid_rewrite Hpsent; saturate_assumptions!...
+        all: auto.
+      * split_and?; match goal with |- forall (_ : _), _ -> ?def _ _ => pick def as_ H' by_ (destruct_and? H) end; 
+          clear H; rename H' into H; setoid_rewrite Hpsent.
+        1-2: intros [ src dst msg used ] Hin%(In_consume_conv_full Hin'). 
+        1-2: destruct Hin as (used' & Hin); specialize (H _ Hin).
+        --eapply (h2l_invariants_id_pre Hstep_ Hw) in H. simpl in H. exact H.
+        --(* byz; TODO slightly repeating *)
+          destruct msg as [ | (v0, cs0) | (v0, nsigs0) ], H.
+          all: constructor; hnf; auto...
+          all: setoid_rewrite Hpsent; saturate_assumptions!...
+          all: destruct_exists; repeat match goal with HH : _ |- _ => apply (In_consume_fwd_full Hin') in HH end.
+          all: eauto.
+        --(* check which packet is consumed this time *)
+          destruct p' as [ src' dst' msg' used' ].
+          hnf in H |- *. intros p Hin%In_consume. simpl in Hin.
+          destruct Hin as [ <- | (Hin & _) ].
+          2: specialize (H _ Hin).
+          1: destruct used'; [ specialize (H _ Hin') | ].
+          1,3: eapply (h2l_invariants_id_pre Hstep_ Hw) in H; simpl in H; exact H.
+          (* interesting part *)
+          clear H. destruct Hb as (Hnonbyz & Hr).
+          destruct msg' as [ v' lsig' sig' | (v', cs') | (v', nsigs') ]; simpl in Hr.
+          all: constructor; try exact I.
+          all: hnf; simpl; auto.
+    + destruct a as [ pkts [ n m ] Hf Hcheck ]. simpl in *. subst pkts.
+      clear Hb. destruct Hpsent as (psent_ & Hpmnt & Hineq), Hse as (Hse & Hnonbyz & Hb).
+      saturate_assumptions!. clear H.
+      split_and?; match goal with |- forall (_ : _), _ -> ?def _ _ => pick def as_ H by_ (destruct_and? IH) end; clear IH.
+      all: intros p Hin%Hineq; autorewrite with psent in Hin.
+      all: try (destruct Hin as [ (dst & ->)%In_broadcast | ]; [ | solve [ intuition ] ]).
+      * (* interesting case *)
+        constructor.
+        all: hnf; destruct m as [ | [] | [] ]; simpl in *; auto.
+      * (* byz; TODO slightly repeating *)
+        rewrite In_broadcast in Hin.
+        destruct Hin as [ (dst & ->) | Hin ]; 
+          [ | specialize (H _ Hin); rename m into m0; destruct p as [ src0 dst0 m used0 ], H ]; 
+          destruct m as [ | (v0, cs0) | (v0, nsigs0) ].
+        all: constructor; hnf; auto; try congruence... (* is_byz conflict *)
+        all: setoid_rewrite Hineq; saturate_assumptions!...
+        all: setoid_rewrite In_sendout.
+        all: destruct_exists; eauto.
+      * constructor; destruct m as [ | [] | [] ]; hnf; auto.
+  - (* byz step; easy? *)
+    destruct Hse as (Hbyz & -> & Hcb), Hpsent as (Els & Hpsent), H as (HHsent & HHbyz & HHrcv). 
+    rewrite Hpsent, Els. clear Els Hpsent.
+    split_and?; intros p; rewrite In_sendout1; intros [ <- | Hin ]; auto.
+    all: constructor; hnf; destruct msg as [ | [] | [] ]; simpl; intros; try solve [ auto | congruence | tauto ].
+    (* now only Byz goals left *)
+    all: clear HHsent HHrcv.
+    all: tryif progress saturate_assumptions! then destruct HHbyz else idtac.
+    (* here, do some manual work to avoid simplify_eq gives wierd substition results *)
+    all: match goal with 
+      | |- (match ?pp with _ => _ end) => destruct pp as [ src0 dst0 [ | [] | [] ] used0 ]; intros; simpl in *; auto; saturate_assumptions
+      | _ => idtac end...
+    all: saturate_assumptions!...
+    all: simpl in *; setoid_rewrite In_sendout1.
+    all: destruct_exists; eauto.
+Qed.
+
+Record node_psent_h2l_invariants_nonbyz p stmap : Prop := {
+  _ : inv_submitmsg_correct p stmap;
+  _ : inv_lightconfirmmsg_correct_nonbyz p stmap;
+  _ : inv_confirmmsg_correct_nonbyz p stmap;
+  _ : inv_submitmsg_receive p stmap;
+  _ : inv_lightconfirmmsg_receive p stmap;
+  _ : inv_confirmmsg_receive p stmap;
+}.
+
+Fact h2l_invariants :
+  always_holds (lift_pkt_inv node_psent_h2l_invariants_nonbyz) /\
+  always_holds (lift_pkt_inv_alt node_psent_h2l_invariants_byz).
+Proof.
+  unshelve epose proof (is_invariant_reachable_step_under_closed _ _ h2l_invariants_pre _ id_coh_always_holds) as H. 
+  - simpl. split_and?; hnf; intros; contradiction.
+  - rewrite !always_holds_and in H. destruct_and? H. split; auto.
+    repeat progress (hnf in *; intros; saturate_assumptions!).
+    pick node_psent_h2l_invariants_sent_nonbyz as_ HH1. 
+    pick node_psent_h2l_invariants_recv_pre as_ HH2.
+    destruct HH1, HH2. constructor; auto.
+    now apply inv_submitmsg_receive_always_holds.
+Qed.
+
+End Backward.
+
+End Main_Proof.
+
+End ACInvariant.
