Protocols/ABC/Nw.v
@@ -1,0 +1,83 @@
+From Coq Require Import List Lia.
+From Coq Require ssrbool ssreflect.
+Import (coercions) ssrbool.
+Import ssreflect.SsrSyntax.
+From ABCProtocol.Systems Require Export Network.
+From ABCProtocol.Protocols.ABC Require Export Pro.
+
+Module ACAdversary (A : NetAddr) (V : Signable) (VBFT : ValueBFT A V) 
+  (BTh : ByzThreshold A) (BSett : ByzSetting A)
+  (P : PKI A V) (TSS : ThresholdSignatureScheme A V with Definition thres := BTh.t0)
+  (ACDT : ACDataTypes A V P TSS) 
+  (CC : CertCheckers A V P TSS ACDT) (M : ACMessage A V P TSS ACDT)
+  (P0 : SimplePacket A M) 
+  (ACP : ACProtocol A V VBFT BTh P TSS ACDT CC M P0) 
+  (Ns : NetState A M P0 BTh ACP) <: Adversary A M BTh BSett P0 ACP Ns.
+
+Import A V VBFT BTh BSett P TSS ACDT CC M P0 ACP Ns.
+
+(* yes, how about extracting this to be ...? *)
+Definition sig_seen_in_history (src : Address) (v : Value) (s : Signature) (pkts : PacketSoup) :=
+  exists dst consumed ls, In (mkP src dst (SubmitMsg v ls s) consumed) pkts.
+
+Definition cert_correct (psent : PacketSoup) (c : Certificate) :=
+  let: (v, nsigs) := c in
+  forall n sig, 
+    In (n, sig) nsigs ->
+    is_byz n = false ->
+    verify v sig n -> (* this can be expressed in other way *)
+    sig_seen_in_history n v sig psent. 
+
+(* TODO the lightsig can actually be obtained from full certificates?
+  guess this will not affect the following reasoning 
+  (since full certificates are assembled from the sent messages), 
+  so ignore it for now *)
+Definition lightsig_seen_in_history (src : Address) (v : Value) (ls : LightSignature) (pkts : PacketSoup) :=
+  exists dst consumed s, In (mkP src dst (SubmitMsg v ls s) consumed) pkts.
+
+(* safety assumption about light certificates: 
+  if the number of Byzantine nodes is not sufficiently large, 
+  then the light signature is unforgeable *)
+(* TODO can we say that the light certificate is unforgeable instead (just like here)? *)
+Definition lcert_correct (psent : PacketSoup) (lc : LightCertificate) : Prop :=
+  let: (v, cs) := lc in
+  combined_verify v cs ->
+  forall lsigs,
+    cs = lightsig_combine lsigs ->
+    forall n lsig,
+      In lsig lsigs ->
+      is_byz n = false ->
+      light_verify v lsig n ->
+      lightsig_seen_in_history n v lsig psent. 
+
+Definition lcert_correct_threshold (psent : PacketSoup) (lc : LightCertificate) : Prop :=
+  (num_byz < N - (thres + thres) -> lcert_correct psent lc).
+
+Definition byz_constraints (m : Message) (w : World) : Prop :=
+  match m with
+  | SubmitMsg v lsig sig => True
+  | LightConfirmMsg lc => lcert_correct_threshold (sentMsgs w) lc
+  | ConfirmMsg c => cert_correct (sentMsgs w) c
+  end.
+
+End ACAdversary.
+
+Module ACNetwork (A : NetAddr) (V : Signable) (VBFT : ValueBFT A V) 
+  (BTh : ByzThreshold A) (BSett : ByzSetting A)
+  (P : PKI A V) (TSS : ThresholdSignatureScheme A V with Definition thres := BTh.t0).
+
+Import A V VBFT BTh BSett P TSS.
+
+Module Export ACDT <: ACDataTypes A V P TSS := ACDataTypesImpl A V P TSS.
+Module Export CC : (* hide implementation *) CertCheckers A V P TSS ACDT := CertCheckersImpl A V P TSS ACDT.
+Module Export M <: MessageType := ACMessageImpl A V P TSS ACDT.
+Module Export P0 <: SimplePacket A M := SimplePacketImpl A M.
+Module Export PSOp : (* hide implementation *) PacketSoupOperations P0 := PacketSoupOperationsImpl P0.
+Module Export ACP <: Protocol A M P0 BTh <: ACProtocol A V VBFT BTh P TSS ACDT CC M P0 :=
+  ACProtocolImpl A V VBFT BTh P TSS ACDT CC M P0.
+Module Export Ns <: NetState A M P0 BTh ACP := NetStateImpl A M P0 BTh ACP.
+Module Export ACAdv <: Adversary A M BTh BSett P0 ACP Ns := ACAdversary A V VBFT BTh BSett P TSS ACDT CC M P0 ACP Ns.
+
+Include NetworkImpl A M BTh BSett P0 PSOp ACP Ns ACAdv.
+
+End ACNetwork.
