Structures/Address.v
@@ -1,4 +1,5 @@
 From Coq Require Import Lia List.
+From ABCProtocol.Utils Require Export Tactics.
 
 Module Type NetAddr.
 
