Utils/Tactics.v
@@ -1,0 +1,106 @@
+From Coq Require ssrbool.
+
+Global Tactic Notation "eqsolve" := solve [ intuition congruence | intuition discriminate ].
+
+Global Tactic Notation "pick" constr(def) "as_" ident(H) :=
+  first
+  [ match goal with
+    | H0 : def _ |- _ => rename H0 into H
+    | H0 : def _ _ |- _ => rename H0 into H
+    | H0 : def _ _ _ |- _ => rename H0 into H
+    end
+  | match goal with
+    | H0 : context[def] |- _ => rename H0 into H; hnf in H
+    end ];
+  tryif (is_const def) then (unfold def in H) else idtac.
+
+(* TODO need improvement *)
+Global Tactic Notation "pick" constr(def) "as_" ident(H) "by_" tactic2(tac) :=
+  let a := fresh "eprop" in
+  evar (a : Prop); assert a as H; subst a; 
+    [ tac; (let Htmp := fresh "Htmp" in pick def as_ Htmp; exact Htmp) | ].
+
+Global Tactic Notation "saturate_assumptions" :=
+  repeat match goal with
+    H : ?P -> ?Q |- _ => 
+    match type of P with
+      Prop => specialize (H ltac:(try apply I; try reflexivity; assumption))
+    end
+  end.
+
+Local Ltac sat H :=
+  match type of H with
+  | forall (_ : ?P), _ =>
+    tryif 
+      ((first [ specialize (H I) | specialize (H eq_refl) | specialize (H ltac:(assumption)) ]; sat H) +
+      (* search with backtracking *)
+      (match goal with
+      | HH : ?P |- _ => specialize (H HH); sat H
+      end)) then idtac else fail 1
+  | _ => idtac
+  end.
+
+(* just a wrapper with a better name *)
+Global Tactic Notation "saturate_assumptions" "!" "in_" hyp(H) := sat H.
+
+Global Tactic Notation "saturate_assumptions" "!" :=
+  repeat match goal with
+  | H : forall (_ : _), _ |- _ => sat H
+  end.
+
+Global Tactic Notation "hypothesis" :=
+  match goal with
+    H : ?e |- _ => 
+    match type of e with
+      Prop => solve [ simple apply H ]
+    end
+  end.
+
+(* FIXME: later, combine the following two together *)
+Global Ltac isSome_rewrite :=
+  repeat match goal with
+  | H : ?a = _, H0 : context[ssrbool.isSome ?a] |- _ => rewrite H in H0; simpl in H0
+  | H : ?a = _ |- context[ssrbool.isSome ?a] => rewrite H; simpl
+  end.
+
+Global Ltac is_true_rewrite :=
+  repeat match goal with
+  | H : ?a = true, H0 : context[is_true ?a] |- _ => rewrite H in H0; change (is_true true) with (true = true) in H0
+  | H : ?a = false, H0 : context[is_true ?a] |- _ => rewrite H in H0; change (is_true false) with (false = true) in H0
+  | H : ?a = true |- context[is_true ?a] => rewrite H; change (is_true true) with (true = true)
+  | H : ?a = false |- context[is_true ?a] => rewrite H; change (is_true false) with (false = true)
+  end.
+
+Global Ltac match_option_rewrite :=
+  repeat match goal with
+  | H : ?a = _, H0 : context[match ?a with Some _ => _ | None => _ end] |- _ => rewrite H in H0; simpl in H0
+  | H : ?a = _ |- context[match ?a with Some _ => _ | None => _ end] => rewrite H; simpl
+  end.
+
+Global Tactic Notation "destruct_eqdec_raw" constr(eqdec) constr(a) constr(b) simple_intropattern(pat) :=
+  match type of eqdec with
+    forall _ : _, forall _ : _, sumbool (eq _ _) (not (eq _ _)) =>
+    destruct (eqdec a b) as [ pat | ] +
+    destruct (eqdec a b) as [ | ]
+  end.
+
+Global Tactic Notation "destruct_eqdec" "in_" hyp(H) "as_" simple_intropattern(pat) :=
+  repeat match type of H with
+    context[if ?eqdec ?a ?b then _ else _] => destruct_eqdec_raw eqdec a b pat
+  end.
+
+Global Tactic Notation "destruct_eqdec" "as_" simple_intropattern(pat) :=
+  repeat match goal with
+    |- context[if ?eqdec ?a ?b then _ else _] => destruct_eqdec_raw eqdec a b pat
+  end.
+
+Global Tactic Notation "destruct_eqdec" "!" "as_" simple_intropattern(pat) :=
+  repeat match goal with 
+  | H : context[if ?eqdec ?a ?b then _ else _] |- _ => destruct_eqdec_raw eqdec a b pat
+  end; try destruct_eqdec as_ pat.
+
+Global Tactic Notation "destruct_exists" :=
+  repeat match goal with
+    H : exists (_ : _), _ |- _ =>
+    destruct H as (? & ?)
+  end.
